refactoring

MathematicalLogic/FirstOrder/Completeness/TermModel.lean
@@ -1,56 +1,98 @@
 import MathematicalLogic.FirstOrder.Semantics
-import MathematicalLogic.FirstOrder.Completeness.Basic
+import MathematicalLogic.FirstOrder.Completeness.Defs
 
-@[reducible] def TermModel (Γ : Context 𝓛) : Structure 𝓛 where
-  𝓤 := Term 𝓛
-  inhabited := ⟨#0⟩
-  𝓕 := λ f ts => f ⬝ₜ ts
-  𝓟 := λ p ts => Γ ⊢ p ⬝ₚ ts
+def Vec.setoid (s : Setoid α) (n : ℕ) : Setoid (Vec α n) where
+  r v₁ v₂ := ∀ i, s.r (v₁ i) (v₂ i)
+  iseqv.refl _ _ := s.iseqv.refl _
+  iseqv.symm h i := s.iseqv.symm (h i)
+  iseqv.trans h₁ h₂ i := s.iseqv.trans (h₁ i) (h₂ i)
 
-local notation "𝓜ᵀ" => TermModel
+instance [s : Setoid α] : Setoid (Vec α n) := Vec.setoid s n
 
-mutual
-theorem Term.interp_term_model :
-  ⟦ t ⟧ₜ 𝓜ᵀ Γ, ρ = t[ρ]ₜ :=
-  match t with
-  | #x => by simp
-  | f ⬝ₜ ts => by simp; rw [Terms.interp_term_model]
-theorem Terms.interp_term_model :
-  (⟦ ts ⟧ₜₛ 𝓜ᵀ Γ, ρ : Terms 𝓛 n) = ts[ρ]ₜₛ :=
-  match ts with
-  | []ₜ => by simp
-  | t ∷ₜ ts => by
-    simp
-    rw [Term.interp_term_model, Terms.interp_term_model]
-    trivial
-end
+def Vec.quotient {s : Setoid α} (v : Vec (Quotient s) n) : Quotient (Vec.setoid s n) :=
+  v.rec ⟦[]ᵥ⟧
+    (λ a _ v => Quotient.liftOn₂ a v (⟦· ∷ᵥ ·⟧)
+      (by
+        intros; simp; intro i
+        cases i using Fin.cases with
+        | zero => assumption
+        | succ => apply_assumption))
 
-lemma subst_const {c : Const 𝓛} : (c : Term 𝓛)[σ]ₜ = c := rfl
+theorem Vec.quotient_mk :
+  quotient (s := s) (λ i => ⟦v i⟧) = ⟦v⟧ := by
+  induction v using Vec.rec with
+  | nil => simp [Vec.eq_nil, quotient]
+  | cons a v ih =>
+    rw [Vec.eq_cons λ _ => _]
+    simp [head, tail, Function.comp, quotient]
+    rw [←quotient]
+    simp [ih]
 
-lemma assignment_cons_in_term_model
-  {Γ : Context 𝓛} {ρ : Assignment (TermModel Γ)} :
-  ⇑ₛρ ∘ₛ ↦ₛ t = Assignment.cons (𝓜 := TermModel Γ) t ρ := by
-  funext x
-  cases x with
-  | zero => rfl
-  | succ x => simp [Subst.comp, Subst.lift, Term.shift_subst_single, Assignment.cons]
+def Quotient.liftOnVec
+  {s : Setoid α}
+  (v : Vec (Quotient s) n)
+  (f : Vec α n → β)
+  (c : (v₁ v₂ : Vec α n) → v₁ ≈ v₂ → f v₁ = f v₂) : β :=
+  Quotient.liftOn v.quotient f c
+
+theorem Quotient.liftOnVec_mk
+  {s : Setoid α} {f : Vec α n → β} {c : (v₁ v₂ : Vec α n) → v₁ ≈ v₂ → f v₁ = f v₂} :
+  liftOnVec (λ i => ⟦v i⟧) f c = f v := by
+  simp [liftOnVec, Vec.quotient_mk, Quotient.liftOn_mk]
+
+
+
+namespace FirstOrder.Language
+
+variable {𝓛 : Language}
+
+namespace Context
+
+variable (Γ : 𝓛.Context)
+
+def TermSetoid : Setoid 𝓛.Term where
+  r p q := Γ ⊢ p ≐ q
+  iseqv.refl _ := Proof.refl
+  iseqv.symm := Proof.symm.mp
+  iseqv.trans := Proof.trans.mp2
+
+@[simps] def TermModel (Γ : 𝓛.Context) : 𝓛.Structure where
+  𝓤 := Quotient Γ.TermSetoid
+  inhabited𝓤 := ⟨⟦#0⟧⟩
+  interp𝓕 f v :=
+    Quotient.liftOnVec v (⟦f ⬝ₜ ·⟧)
+      (by intros v₁ v₂ h; simp; papply Proof.congr_func; exact Proof.andN_intro h)
+  interp𝓡 r v :=
+    Quotient.liftOnVec v (Γ ⊢ r ⬝ᵣ ·)
+      (by intros v₁ v₂ h; simp; apply Proof.iff_iff; papply Proof.congr_rel_iff; exact Proof.andN_intro h)
+
+end Context
+
+variable {Γ : 𝓛.Context} {ρ : 𝓛.Subst}
+
+theorem Term.interp_term_model : ⟦ t ⟧ₜ Γ.TermModel, (⟦ρ ·⟧) = ⟦t[ρ]ₜ⟧ := by
+  induction t with simp [Term.interp]
+  | func f v ih => simp [ih, Quotient.liftOnVec_mk]
+
+lemma subst_const {c : 𝓛.Const} : (c : 𝓛.Term)[σ]ₜ = c := by simp; apply Vec.eq_nil
+
+variable  (h₁ : Γ.Consistent) (h₂ : Γ.Complete) (h₃ : Γ.Saturated)
 
 theorem Formula.interp_term_model :
-  MaximalConsistent Γ → WitnessProperty Γ →
-  (⟦ p ⟧ₚ 𝓜ᵀ Γ, ρ ↔ Γ ⊢ p[ρ]ₚ) := by
-  rintro ⟨h₁, h₂⟩ h₃
-  induction p generalizing ρ <;> simp
-  case atom p ts => simp [Terms.interp_term_model]
-  case fal => exact h₁
-  case imp p q ih₁ ih₂ =>
+  (Γ.TermModel ⊨[(⟦ρ ·⟧)] p ↔ Γ ⊢ p[ρ]ₚ) := by
+  induction p generalizing ρ with simp [Formula.interp]
+  | rel r v => simp [Term.interp_term_model, Quotient.liftOnVec_mk]
+  | eq t₁ t₂ => simp [Term.interp_term_model]; rfl
+  | false => exact h₁
+  | imp p q ih₁ ih₂ =>
     rw [ih₁, ih₂]
     constructor
     · intro h
       rcases h₂ (p[ρ]ₚ) with h' | h'
-      · exact Proof.mp (Proof.axioms Axioms.a1) (h h')
-      · exact Proof.mp Proof.contradiction h'
+      · pintro; pexact (h h')
+      · papply Proof.contradiction; exact h'
     · exact Proof.mp
-  case all p ih =>
+  | all p ih =>
     constructor
     · intro h₁'
       rcases h₂ (∀' p[⇑ₛρ]ₚ) with h₂' | h₂'
@@ -59,23 +101,27 @@ theorem Formula.interp_term_model :
         apply Proof.mp Proof.not_forall at h₂'
         apply h₃ at h₂'
         rcases h₂' with ⟨c, h₂'⟩
-        simp [Formula.subst, Formula.subst_comp] at h₂'
-        rw [←subst_const (σ := ρ)] at h₂'
+        simp at h₂'; rw [←subst_const (σ := ρ), ←Formula.subst_swap, ←Formula.subst_comp] at h₂'
         apply h₁
-        apply Proof.mp h₂'
-        rw [←ih, assignment_cons_in_term_model]
+        apply h₂'.mp
+        simp [←ih]
+        have : (λ x => ⟦(↦ₛ c x)[ρ]ₜ⟧) = Structure.Assignment.cons (𝓢 := Γ.TermModel) ⟦c⟧ (⟦ρ ·⟧) := by
+          funext x; cases x <;> simp [Structure.Assignment.cons, Vec.eq_nil]
+        rw [this]
         apply h₁'
-    · intros h t
-      apply Proof.mp (Proof.axioms (Axioms.a4 (t := t))) at h
-      rw [Formula.subst_comp, ←ih, assignment_cons_in_term_model] at h
+    · rintro h ⟨t⟩
+      apply Proof.mp (Proof.ax (.a4 (t := t))) at h
+      rw [←Formula.subst_comp, ←ih] at h
+      have : (λ x => ⟦(⇑ₛρ ∘ₛ ↦ₛ t) x⟧) = Structure.Assignment.cons (𝓢 := Γ.TermModel) ⟦t⟧ (⟦ρ ·⟧) := by
+        funext x; cases x <;> simp [Structure.Assignment.cons, Term.shift_subst_single]
+      rw [this] at h
       exact h
 
-theorem satisfiable_by_term_model :
-  MaximalConsistent Γ → WitnessProperty Γ → Satisfiable Γ := by
-  intros h₁ h₂
-  apply Satisfiable.up.{0}
-  exists 𝓜ᵀ Γ, idₛ
+theorem satisfiable_by_term_model : Γ.Satisfiable := by
+  apply Context.Satisfiable.up.{0}
+  exists Γ.TermModel, (⟦Subst.id ·⟧)
   intros p h
-  rw [Formula.interp_term_model h₁ h₂, Formula.subst_id]
-  apply Proof.assumption
-  exact h
+  rw [Formula.interp_term_model h₁ h₂ h₃, Formula.subst_id]
+  exact Proof.hyp h
+
+end FirstOrder.Language
