MathematicalLogic/FirstOrder/Proof.lean
@@ -1,176 +1,246 @@
 import Mathlib.Data.Set.Finite
 import MathematicalLogic.FirstOrder.Syntax
 
-@[reducible] def Context (𝓛) := Set (Formula 𝓛)
+namespace FirstOrder.Language
 
-def Context.append (Γ : Context 𝓛) (p) := insert p Γ
-infixl:51 ",' " => Context.append
+variable {𝓛 : Language}
 
-def Context.lift : Context 𝓛 → Context 𝓛 := λ Γ => {↑ₚp | p ∈ Γ}
-prefix:max "↑ₚₛ" => Context.lift
+abbrev Context (𝓛 : Language) := Set 𝓛.Formula
 
-theorem Context.lift_append : ↑ₚₛ(Γ,' p) = ↑ₚₛΓ,' ↑ₚp := Set.image_insert_eq
+def Context.append (Γ : 𝓛.Context) (p) := insert p Γ
+infixl:51 ",, " => Context.append
 
-inductive Axioms (𝓛) : Context 𝓛 where
-| a1 : Axioms 𝓛 (p ⇒ (q ⇒ p))
-| a2 : Axioms 𝓛 ((p ⇒ q ⇒ r) ⇒ (p ⇒ q) ⇒ p ⇒ r)
-| a3 : Axioms 𝓛 ((~ p ⇒ ~ q) ⇒ q ⇒ p)
-| a4 : Axioms 𝓛 (∀' p ⇒ p[↦ₛ t]ₚ)
-| a5 : Axioms 𝓛 (p ⇒ ∀' ↑ₚp)
-| a6 : Axioms 𝓛 (∀' (p ⇒ q) ⇒ ∀' p ⇒ ∀' q)
-| a7 : Axioms 𝓛 p → Axioms 𝓛 (∀' p)
+def Context.lift : 𝓛.Context → 𝓛.Context := λ Γ => {↑ₚp | p ∈ Γ}
+prefix:max "↑ᶜ" => Context.lift
+theorem Context.lift_append : ↑ᶜ(Γ,, p) = ↑ᶜΓ,, ↑ₚp := Set.image_insert_eq
 
-inductive Proof (Γ : Context 𝓛) : Formula 𝓛 → Prop where
-| assumption : p ∈ Γ → Proof Γ p
-| axioms : p ∈ Axioms 𝓛 → Proof Γ p
+inductive Axioms (𝓛 : Language) : 𝓛.Context where
+| a1 {p q : 𝓛.Formula} :
+  𝓛.Axioms (p ⇒ (q ⇒ p))
+| a2 {p q r : 𝓛.Formula} :
+  𝓛.Axioms ((p ⇒ q ⇒ r) ⇒ (p ⇒ q) ⇒ p ⇒ r)
+| a3 {p q : 𝓛.Formula} :
+  𝓛.Axioms ((~ p ⇒ ~ q) ⇒ q ⇒ p)
+| a4 {t : 𝓛.Term} {p : 𝓛.Formula} :
+  𝓛.Axioms (∀' p ⇒ p[↦ₛ t]ₚ)
+| a5 {p : 𝓛.Formula} :
+  𝓛.Axioms (p ⇒ ∀' ↑ₚp)
+| a6 {p q : 𝓛.Formula} :
+  𝓛.Axioms (∀' (p ⇒ q) ⇒ ∀' p ⇒ ∀' q)
+| e1 {t : 𝓛.Term} :
+  𝓛.Axioms (t ≐ t)
+| e2 {t₁ t₂ : 𝓛.Term} {p : 𝓛.Formula} :
+  𝓛.Axioms ((t₁ ≐ t₂) ⇒ p[↦ₛ t₁]ₚ ⇒ p[↦ₛ t₂]ₚ)
+| all {p : 𝓛.Formula} :
+  𝓛.Axioms p → 𝓛.Axioms (∀' p)
+
+theorem Axioms.closed_under_subst : p ∈ 𝓛.Axioms → p[σ]ₚ ∈ 𝓛.Axioms := by
+  intro h
+  induction h generalizing σ
+    <;> simp [Formula.subst_swap, Formula.shift_subst_lift]
+  case all ih => exact all ih
+  all_goals constructor
+
+inductive Proof (Γ : 𝓛.Context) : 𝓛.Formula → Prop where
+| hyp : p ∈ Γ → Proof Γ p
+| ax : p ∈ 𝓛.Axioms → Proof Γ p
 | mp : Proof Γ (p ⇒ q) → Proof Γ p → Proof Γ q
-
 infix:50 " ⊢ " => Proof
 
 namespace Proof
 
+variable {Γ Δ : 𝓛.Context} {t t₁ t₂ : 𝓛.Term} {p q r : 𝓛.Formula}
+
+theorem hyp_append : Γ,, p ⊢ p :=
+  hyp (Set.mem_insert _ _)
+
 theorem weaken : Γ ⊆ Δ → Γ ⊢ p → Δ ⊢ p := by
   intros h₁ h₂
   induction h₂ with
-  | assumption h => exact assumption (h₁ h)
-  | axioms h => exact axioms h
+  | hyp h => exact hyp (h₁ h)
+  | ax h => exact ax h
   | mp _ _ ih₁ ih₂ => exact mp ih₁ ih₂
 
-theorem weaken_add : Γ ⊢ p → Γ,' q ⊢ p := by
-  apply weaken
-  apply Set.subset_insert
+theorem weaken_append : Γ ⊢ p → Γ,, q ⊢ p :=
+  weaken (Set.subset_insert _ _)
 
 theorem mp2 : Γ ⊢ p ⇒ q ⇒ r → Γ ⊢ p → Γ ⊢ q → Γ ⊢ r :=
   λ h₁ h₂ h₃ => mp (mp h₁ h₂) h₃
 
 theorem identity : Γ ⊢ p ⇒ p :=
-  mp2 (axioms Axioms.a2) (axioms Axioms.a1) (axioms (Axioms.a1 (q := p)))
+  mp2 (ax .a2) (ax .a1) (ax (.a1 (q := p)))
 
-theorem deduction : Γ ⊢ p ⇒ q ↔ Γ,' p ⊢ q := by
+theorem deduction : Γ ⊢ p ⇒ q ↔ Γ,, p ⊢ q := by
   constructor
-  · intro h
-    apply mp
-    · apply weaken
-      · apply Set.subset_union_right
-      · exact h
-    · apply assumption
-      left
-      rfl
+  · intro h; exact mp (weaken_append h) hyp_append
   · intro h
     induction h with
-    | assumption h =>
-      simp at h
+    | hyp h =>
       cases h with
-      | inl h => cases h; apply identity
-      | inr h => exact mp (axioms Axioms.a1) (assumption h)
-    | axioms h => exact mp (axioms Axioms.a1) (axioms h)
-    | mp _ _ ih₁ ih₂ => exact mp (mp (axioms Axioms.a2) ih₁) ih₂
+      | inl h => subst h; exact identity
+      | inr h => exact mp (ax .a1) (hyp h)
+    | ax h => exact mp (ax .a1) (ax h)
+    | mp _ _ ih₁ ih₂ => exact mp (mp (ax .a2) ih₁) ih₂
 
-macro "repeatn" n:num t:tactic : tactic => do
-  let mut t' ← `(tactic| skip)
-  for _ in [:n.getNat] do
-    t' ← `(tactic| ($t'; $t))
-  return t'
+theorem cut : Γ ⊢ p → Γ,, p ⊢ q → Γ ⊢ q :=
+  λ h₁ h₂ => mp (deduction.mpr h₂) h₁
 
-macro "passumption" : tactic =>
-  `(tactic| (
-    apply assumption
-    repeat first | exact Or.inl rfl | apply Or.inr
-  ))
+lemma closed_under_subst : Γ ⊢ p → { q[σ]ₚ | q ∈ Γ } ⊢ p[σ]ₚ := by
+  intro h
+  induction h with
+  | hyp h => apply hyp; exists _, h
+  | ax h => exact ax (Axioms.closed_under_subst h)
+  | mp _ _ ih₁ ih₂ => exact mp ih₁ ih₂
 
-macro "passumption" n:num : tactic =>
-  `(tactic| (
-    apply assumption
-    repeatn $n apply Or.inr
-    exact Or.inl rfl
-  ))
-
-macro "pweaken_ctx" : tactic =>
-  `(tactic| (
-    intro _ h
-    try exact h
-    repeat
-      apply Set.subset_insert; try exact h
-  ))
-
-macro "papply" t:term : tactic =>
-  `(tactic| (
-    first
-    | apply mp $t
-    | apply mp2 $t
-    | apply λ h₁ h₂ h₃ => mp (mp (mp $t h₁) h₂) h₃
-    | apply λ h₁ h₂ h₃ h₄ => mp (mp (mp (mp $t h₁) h₂) h₃) h₄
-  ))
-
-macro "papplyw" t:term : tactic =>
-  `(tactic| (
-    first
-    | apply mp (weaken (by pweaken_ctx) $t)
-    | apply mp2 (weaken (by pweaken_ctx) $t)
-    | apply λ h₁ h₂ h₃ => mp (mp (mp (weaken (by pweaken_ctx) $t) h₁) h₂) h₃
-    | apply λ h₁ h₂ h₃ h₄ => mp (mp (mp (mp (weaken (by pweaken_ctx) $t) h₁) h₂) h₃) h₄
-  ))
-
-macro "papply_assumption" n:num : tactic =>
-  `(tactic| papply (by passumption $n))
-
-macro "papply" n:num : tactic =>
-  `(tactic| (
-    first
-    | apply mp; passumption $n
-    | apply mp2; passumption $n
-    | apply λ h h₁ h₂ h₃ => mp (mp (mp h h₁) h₂) h₃; passumption $n
-    | apply λ h h₁ h₂ h₃ h₄ => mp (mp (mp (mp h h₁) h₂) h₃) h₄; passumption $n
-  ))
+theorem closed_under_shift : Γ ⊢ p → ↑ᶜΓ ⊢ ↑ₚp := closed_under_subst
 
 macro "pintro" : tactic => `(tactic| apply deduction.mpr)
-macro "pintros" : tactic => `(tactic| repeat pintro)
-macro "pintros" n:num : tactic => `(tactic| repeatn $n pintro)
+elab "pintros" n:(ppSpace colGt num)? : tactic => do
+  match n with
+  | some n =>
+    for _ in [:n.getNat] do
+      Lean.Elab.Tactic.evalTactic (←`(tactic| pintro))
+  | none =>
+    Lean.Elab.Tactic.evalTactic (←`(tactic| repeat pintro))
 
-theorem psuffices (h₁ : Γ,' p ⊢ q) (h₂ : Γ ⊢ p) : Γ ⊢ q :=
-  mp (deduction.mpr h₁) h₂
-theorem phave (h₁ : Γ ⊢ p) (h₂ : Γ,' p ⊢ q) : Γ ⊢ q :=
-  mp (deduction.mpr h₂) h₁
-macro "psuffices" t:term : tactic => `(tactic| apply psuffices (p := $t))
-macro "phave" t:term : tactic => `(tactic| apply phave (p := $t) )
+private def hypTerm (n : ℕ) : Lean.MacroM (Lean.TSyntax `term) := do
+  let mut t ← `(hyp_append)
+  for _ in [:n] do
+    t ← `(weaken_append $t)
+  return t
+
+macro "passumption" n:(ppSpace colGt num)? : tactic => do
+  match n with
+  | some n => `(tactic| exact $(← hypTerm n.getNat))
+  | none => `(tactic| (apply hyp; repeat first | exact Or.inl rfl | apply Or.inr))
+
+macro "phave" t:(ppSpace colGt term) : tactic =>
+  `(tactic| refine cut (p := $t) ?_ ?_)
+macro "psuffices" t:(ppSpace colGt term) : tactic =>
+  `(tactic| (refine cut (p := $t) ?_ ?_; swap))
+
+/--
+  Unify `Γ ⊆ Δ` as `Γ, p₁, ⋯, pₙ = Δ`.
+  Return `some n` if succeed, and `none` if fail. -/
+private partial def isSubsetOf (Γ Δ : Lean.Expr) : Lean.MetaM (Option ℕ) := do
+  let s ← Lean.MonadBacktrack.saveState
+  if ← Lean.Meta.isDefEq Γ Δ then
+    return some 0
+  Lean.MonadBacktrack.restoreState s
+  if let some (_, Δ', _) := Δ.app3? ``Context.append then
+    if let some n := ← isSubsetOf Γ Δ' then
+      return some (n + 1)
+  return none
+
+/--
+  Given a proof term of `Γ ⊢ p₁ ⇒ ⋯ ⇒ pₙ`, apply it on the goal `Γ' ⊢ pₙ` through MP.
+  `Γ` should be a subset of `Γ'`.
+  
+  Control the application depth `n` through `with` clause. -/
+elab "papply" t:(ppSpace colGt term) d:((" with " num)?) : tactic =>
+  Lean.Elab.Tactic.withMainContext do
+    let appTerm ← Lean.Elab.Term.elabTerm t none
+    let appType ← Lean.instantiateMVars (← Lean.Meta.inferType appTerm)
+    let (forallMVars, _, type) ← Lean.Meta.forallMetaTelescopeReducing appType
+    let (Lean.mkApp3 (.const ``Proof []) 𝓛 Γ p) := type
+      | throwError m!"{type} is not a proof"
+    let goal ← Lean.Elab.Tactic.getMainGoal
+    let goalType ← goal.getType'
+    let some (𝓛', Δ, _) := goalType.app3? ``Proof
+      | throwError m!"{goalType} is not a proof"
+    let true := ← Lean.Meta.isDefEq 𝓛 𝓛'
+      | throwError m!"failed to unify {𝓛} and {𝓛'}"
+    let some weakenDepth := ← isSubsetOf Γ Δ
+      | throwError m!"failed to unify {Γ} as a subset of {Δ}"
+    let weakenTy ← do
+      let weakenTy := Lean.mkApp3
+        (.const ``Set.Subset [0]) (.app (.const ``Formula []) 𝓛) Γ Δ
+      Lean.Meta.checkTypeIsProp weakenTy
+      pure weakenTy
+    let weakenTerm ← do
+      let mut weakenTerm ← `(Set.Subset.refl _)
+      for _ in [:weakenDepth] do
+        weakenTerm := ← `(Set.Subset.trans $weakenTerm (Set.subset_insert _ _))
+      Lean.Elab.Term.elabTerm weakenTerm (some weakenTy)
+    let mut proofTerm := Lean.mkApp6
+      (.const ``weaken []) 𝓛 Γ Δ p weakenTerm
+      (Lean.mkAppN appTerm forallMVars)
+    let mut newMVarIds := []
+    let mut goalFormula := p
+    let maxDepth := d.raw.getArgs[1]?.map (·.toNat)
+    repeat do
+      let proofType ← Lean.Meta.inferType proofTerm
+      if ← Lean.Meta.isDefEq goalType proofType then
+        goal.assign proofTerm
+        break
+      if let some d := maxDepth then
+        if newMVarIds.length >= d then
+          throwError "failed to apply {appType} at {goalType} within depth {d}"
+      else if let some (_, p, q) := (← Lean.Meta.whnf goalFormula).app3? ``Formula.imp then
+        let mvarId ← Lean.mkFreshMVarId
+        newMVarIds := newMVarIds ++ [mvarId]
+        let mvar ← Lean.Meta.mkFreshExprMVarWithId mvarId (some (
+          Lean.mkApp3 (.const ``Proof []) 𝓛 Δ p))
+        let newProofTerm := Lean.mkApp6
+          (.const ``mp []) 𝓛 Δ p q proofTerm mvar
+        proofTerm := newProofTerm
+        goalFormula := q
+      else
+        throwError "failed to apply {appType} at {goalType}"
+    for mvar in forallMVars do
+      if let (.mvar mvarid) := mvar then
+        if !(← mvarid.isAssigned) then
+          newMVarIds := newMVarIds ++ [mvarid]
+    Lean.Elab.Tactic.replaceMainGoal newMVarIds
+
+/-- Apply an assumption through MP. -/
+macro "papplya" n:(ppSpace colGt num) : tactic => do
+  `(tactic| papply $(← hypTerm n.getNat))
+
+/-- Close the goal with given proof term. -/
+macro "pexact" t:(ppSpace colGt term) : tactic =>
+  `(tactic| papply $t with 0)
 
 theorem composition : Γ ⊢ (p ⇒ q) ⇒ (q ⇒ r) ⇒ p ⇒ r := by
   pintros
-  papply_assumption 1
-  papply 2
+  papplya 1
+  papplya 2
   passumption
 
 theorem contraposition : Γ ⊢ (p ⇒ q) ⇒ ~ q ⇒ ~ p := composition
+
 theorem contraposition2 : Γ ⊢ (p ⇒ ~ q) ⇒ q ⇒ ~ p := by
   pintros
-  papply 2 <;> passumption
+  papplya 2 <;> passumption
 
 theorem true_intro : Γ ⊢ ⊤ := identity
 
-theorem false_elim : Γ ⊢ ⊥ ⇒ p := mp (axioms Axioms.a3) (mp (axioms Axioms.a1) true_intro)
+theorem false_elim : Γ ⊢ ⊥ ⇒ p := by
+  papply ax .a3
+  pintro
+  exact true_intro
 
 theorem contradiction : Γ ⊢ ~ p ⇒ p ⇒ q := by
   pintros
   papply false_elim
-  papply 1
+  papplya 1
   passumption
 
 theorem double_neg1 : Γ ⊢ p ⇒ ~ ~ p := by
   pintros
-  papply 0
+  papplya 0
   passumption
 
 theorem double_neg2 : Γ ⊢ ~ ~ p ⇒ p := by
   pintro
-  papply axioms Axioms.a3
-  · pintros
-    apply mp <;> passumption
+  papply ax .a3
+  · exact double_neg1
   · passumption
 
 theorem contraposition3 : Γ ⊢ (~ p ⇒ q) ⇒ ~ q ⇒ p := by
   papply composition
   · exact contraposition
-  · papply (axioms Axioms.a2)
+  · papply ax .a2
     pintro
     exact double_neg2
 
@@ -183,178 +253,443 @@ theorem not_imp_left : Γ ⊢ ~ (p ⇒ q) ⇒ p := by
 
 theorem not_imp_right : Γ ⊢ ~ (p ⇒ q) ⇒ ~ q := by
   papply contraposition
-  exact Proof.axioms Axioms.a1
+  exact ax .a1
 
-theorem and_intro : Γ ⊢ p ⇒ q ⇒ p ⋀ q := by
+theorem and_intro : Γ ⊢ p ⇒ q ⇒ p ⩑ q := by
   pintros
-  apply mp2 <;> passumption
+  papplya 0 <;> passumption
 
-theorem and_left : Γ ⊢ p ⋀ q ⇒ p := by
+theorem and_left : Γ ⊢ p ⩑ q ⇒ p := by
   pintro
   papply double_neg2
   pintro
-  papply 1
-  pintros
-  apply mp <;> passumption
-
-theorem and_right : Γ ⊢ p ⋀ q ⇒ q := by
-  pintro
-  apply mp double_neg2
-  pintro
-  papply 1
-  pintro
-  passumption
-
-theorem or_inl : Γ ⊢ p ⇒ p ⋁ q := by
+  papplya 1
   pintros
   papply false_elim
-  apply mp <;> passumption
-
-theorem or_inr : Γ ⊢ q ⇒ p ⋁ q := by
-  pintros
+  papplya 2
   passumption
 
-theorem or_elim : Γ ⊢ p ⋁ q ⇒ (p ⇒ r) ⇒ (q ⇒ r) ⇒ r := by
+theorem and_right : Γ ⊢ p ⩑ q ⇒ q := by
+  pintro
+  papply double_neg2
+  pintro
+  papplya 1
+  pintro
+  passumption
+
+theorem or_inl : Γ ⊢ p ⇒ p ⩒ q := by
+  pintros
+  papply contradiction <;> passumption
+
+theorem or_inr : Γ ⊢ q ⇒ p ⩒ q := ax .a1
+
+theorem or_elim : Γ ⊢ p ⩒ q ⇒ (p ⇒ r) ⇒ (q ⇒ r) ⇒ r := by
   pintros
   papply double_neg2
   pintro
-  papply 0
-  papply 2
-  papply (axioms Axioms.a3)
-  · apply mp2 composition
-    · passumption
-    · apply mp2 composition
-      · passumption
-      · apply double_neg1
-  · passumption
+  papplya 0
+  papplya 2
+  psuffices ~ p
+  · papply contradiction
+    · passumption 1
+    · papplya 2
+      papplya 4
+      passumption
+  · pintro
+    papplya 1
+    papplya 3
+    passumption
 
-theorem excluded_middle : Γ ⊢ ~ p ⋁ p := double_neg2
+theorem excluded_middle : Γ ⊢ ~ p ⩒ p := double_neg2
+
+theorem andN_intro {v : Vec 𝓛.Formula n} :
+  (∀ i, Γ ⊢ v i) → Γ ⊢ ⋀i, v i := by
+  intro h
+  induction n with
+  | zero => exact true_intro
+  | succ n ih =>
+    papply and_intro
+    · apply h
+    · apply ih; intro i; apply h
+
+theorem andN_elim {v : Vec 𝓛.Formula n} {i : Fin n} :
+  (Γ ⊢ ⋀i, v i) → Γ ⊢ v i := by
+  intro h
+  induction n with
+  | zero => exact i.elim0
+  | succ n ih =>
+    cases i using Fin.cases with
+    | zero => exact mp and_left h
+    | succ i => apply ih (mp and_right h)
+
 theorem iff_intro : Γ ⊢ (p ⇒ q) ⇒ (q ⇒ p) ⇒ (p ⇔ q) := and_intro
-theorem iff_left : Γ ⊢ (p ⇔ q) ⇒ (p ⇒ q) := and_left
-theorem iff_right : Γ ⊢ (p ⇔ q) ⇒ (q ⇒ p) := and_right
+theorem iff_mp : Γ ⊢ (p ⇔ q) ⇒ (p ⇒ q) := and_left
+theorem iff_mpr : Γ ⊢ (p ⇔ q) ⇒ (q ⇒ p) := and_right
+theorem iff_iff : Γ ⊢ p ⇔ q → (Γ ⊢ p ↔ Γ ⊢ q) := λ h => ⟨iff_mp.mp2 h, iff_mpr.mp2 h⟩
 
 theorem iff_refl : Γ ⊢ p ⇔ p := mp2 iff_intro identity identity
+
 theorem iff_symm : Γ ⊢ (p ⇔ q) ⇒ (q ⇔ p) := by
   pintro
   papply iff_intro
-  · papply iff_right; passumption
-  · papply iff_left; passumption
+  · papply iff_mpr; passumption
+  · papply iff_mp; passumption
+
 theorem iff_trans : Γ ⊢ (p ⇔ q) ⇒ (q ⇔ r) ⇒ (p ⇔ r) := by
   pintros 2
-  papply iff_intro <;> apply mp2 composition
-  · papply iff_left; passumption
-  · papply iff_left; passumption
-  · papply iff_right; passumption
-  · papply iff_right; passumption
+  papply iff_intro
+  · papply composition <;> papply iff_mp <;> passumption
+  · papply composition <;> papply iff_mpr <;> passumption
+
 theorem iff_congr_imp : Γ ⊢ (p₁ ⇔ p₂) ⇒ (q₁ ⇔ q₂) ⇒ ((p₁ ⇒ q₁) ⇔ (p₂ ⇒ q₂)) := by
   pintros 2
   papply iff_intro <;> pintros
-  · papply iff_left; passumption
-    papply 1
-    papply iff_right; passumption
+  · papply iff_mp; passumption
+    papplya 1
+    papply iff_mpr; passumption
     passumption
-  · papply iff_right; passumption
-    papply 1
-    papply iff_left; passumption
+  · papply iff_mpr; passumption
+    papplya 1
+    papply iff_mp; passumption
     passumption
 
-theorem generalization : ↑ₚₛΓ ⊢ p → Γ ⊢ ∀' p := by
+theorem generalization : ↑ᶜΓ ⊢ p → Γ ⊢ ∀' p := by
   intro h
   induction h with
-  | assumption h =>
+  | hyp h =>
     rcases h with ⟨p, ⟨h₁, h₂⟩⟩
     subst h₂
-    exact mp (axioms Axioms.a5) (assumption h₁)
-  | axioms h => exact axioms (Axioms.a7 h)
-  | mp _ _ ih₁ ih₂ => exact mp2 (axioms Axioms.a6) ih₁ ih₂
+    exact mp (ax .a5) (hyp h₁)
+  | ax h => exact ax (.all h)
+  | mp _ _ ih₁ ih₂ => exact mp2 (ax .a6) ih₁ ih₂
+
+theorem generalization_iff : ↑ᶜΓ ⊢ p ↔ Γ ⊢ ∀' p := by
+  constructor
+  · exact generalization
+  · intro h
+    apply closed_under_shift at h
+    simp [Formula.shift] at h
+    apply mp (ax $ .a4 (t := #0)) at h
+    have : p[⇑ₛSubst.shift]ₚ[↦ₛ #0]ₚ = p := by
+      rw [←Formula.subst_comp]
+      conv => rhs; rw [←Formula.subst_id (p := p)]
+      congr; funext x; cases x <;> simp
+    rw [this] at h
+    exact h
+
+theorem iff_congr_forall : Γ ⊢ ∀' (p ⇔ q) ⇒ ∀' p ⇔ ∀' q := by
+  pintro
+  papply iff_intro <;> papply ax .a6 <;> rw [←deduction] <;> papply ax .a6
+    <;> apply generalization
+  · exact iff_mp
+  · exact iff_mpr
 
 theorem not_forall : Γ ⊢ ~ ∀' p ⇒ ∃' (~ p) := by
   papply contraposition
-  papply (axioms Axioms.a6)
+  papply ax .a6
   apply generalization
-  apply weaken
-  · apply Set.empty_subset
-  · apply double_neg2
+  exact double_neg2
 
 theorem not_exists : Γ ⊢ ~ ∃' p ⇒ ∀' (~ p) := double_neg2
 
-theorem forall_elim : Γ ⊢ ∀' p ⇒ p[↦ₛ t]ₚ := axioms Axioms.a4
+theorem forall_elim : Γ ⊢ ∀' p ⇒ p[↦ₛ t]ₚ := ax .a4
 
 theorem exists_intro : Γ ⊢ p[↦ₛ t]ₚ ⇒ ∃' p := by
   pintros
-  suffices h : _ ⊢ (~ p)[↦ₛ t]ₚ by
-    papply h
+  suffices _ ⊢ (~ p)[↦ₛ t]ₚ by
+    papply this
     passumption
-  papply (axioms Axioms.a4)
+  papply ax .a4
   passumption
 
 theorem exists_elim : Γ ⊢ ∃' p ⇒ (∀' (p ⇒ ↑ₚq)) ⇒ q := by
   pintros
   papply double_neg2
   pintros
-  papply 2
-  suffices h : _ ⊢ ∀' (↑ₚ(~ q) ⇒ ~ p) by
-    apply mp2 (axioms Axioms.a6) h
-    papply (axioms Axioms.a5)
-    passumption
-  papply (axioms Axioms.a6)
+  papplya 2
+  suffices _ ⊢ ∀' (↑ₚ(~ q) ⇒ ~ p) by
+    papply ax .a6
+    · exact this
+    · papply ax .a5
+      passumption
+  papply ax .a6
   · apply generalization
     exact contraposition
   · passumption
 
 theorem exists_self : Γ ⊢ ∃' ↑ₚp ⇒ p := by
   papply contraposition3
-  apply axioms Axioms.a5
+  apply ax .a5
+
+theorem foralls_elim {p : 𝓛.BFormula m} :
+  Γ ⊢ (∀* p).val ⇒ p.val[σ]ₚ := by
+  induction' m with m ih generalizing σ
+  · rw [Sentence.val_subst_eq]; exact identity
+  · let σ' := λ x => σ (x + 1)
+    papply composition
+    · exact ih (σ := σ')
+    · have h : ⇑ₛσ' ∘ₛ ↦ₛ (σ 0) = σ := by
+        funext x; cases x <;> simp [Term.shift_subst_single]
+      conv in _[σ]ₚ => rw [←h, Formula.subst_comp]
+      apply Proof.forall_elim
+
+theorem foralls_elim_self {p : 𝓛.BFormula m} :
+  Γ ⊢ (∀* p).val ⇒ p.val := by
+  rw [←Formula.subst_id (p := p.val)]
+  exact foralls_elim
+
+theorem refl : Γ ⊢ t ≐ t := ax .e1
+macro "prefl" : tactic => `(tactic| pexact refl)
+
+theorem subst : Γ ⊢ t₁ ≐ t₂ ⇒ p[↦ₛ t₁]ₚ ⇒ p[↦ₛ t₂]ₚ := ax .e2
+
+theorem symm : Γ ⊢ t₁ ≐ t₂ ⇒ t₂ ≐ t₁ := by
+  have h := @subst _ Γ t₁ t₂ (#0 ≐ ↑ₜt₁)
+  simp [Term.shift_subst_single] at h
+  pintro
+  papply h
+  · passumption
+  · prefl
+macro "psymm" : tactic => `(tactic| papply symm)
+
+theorem trans : Γ ⊢ t₁ ≐ t₂ ⇒ t₂ ≐ t₃ ⇒ t₁ ≐ t₃ := by
+  have h := @subst _ Γ t₂ t₁ (#0 ≐ ↑ₜt₃)
+  simp [Term.shift_subst_single] at h
+  pintros
+  papply h
+  · psymm; passumption
+  · passumption
+macro "ptrans" t:(ppSpace colGt term)? : tactic =>
+  match t with
+  | some t => `(tactic| papply trans (t₂ := $t))
+  | none => `(tactic| papply trans)
+
+theorem subst_iff : Γ ⊢ t₁ ≐ t₂ ⇒ p[↦ₛ t₁]ₚ ⇔ p[↦ₛ t₂]ₚ := by
+  pintro
+  papply iff_intro <;> papply subst
+  · passumption
+  · psymm; passumption
+
+theorem subst_term : Γ ⊢ t₁ ≐ t₂ ⇒ t[↦ₛ t₁]ₜ ≐ t[↦ₛ t₂]ₜ := by
+  pintro
+  have h := @subst _ Γ t₁ t₂ (↑ₜ(t[↦ₛ t₁]ₜ) ≐ t)
+  simp [Term.shift_subst_single] at h
+  papply h
+  · passumption
+  · prefl
+
+theorem congr_func {v₁ v₂ : Vec 𝓛.Term n} :
+  Γ ⊢ (⋀i, v₁ i ≐ v₂ i) ⇒ f ⬝ₜ v₁ ≐ f ⬝ₜ v₂ := by
+  pintro
+  suffices ∀ k ≤ n, _ ⊢ f ⬝ₜ v₁ ≐ f ⬝ₜ (λ i => if i < k then v₂ i else v₁ i) by
+    replace this := this n (by rfl)
+    simp at this
+    exact this
+  intros k h₁
+  induction k with
+  | zero => simp; prefl
+  | succ k ih =>
+    ptrans
+    · exact ih (Nat.le_of_succ_le h₁)
+    · let k' : Fin n := ⟨k, h₁⟩
+      let t := f ⬝ₜ (λ i => if i < k then ↑ₜ(v₂ i) else if i = k then #0 else ↑ₜ(v₁ i))
+      have h₂ : t[↦ₛ (v₁ k')]ₜ = f ⬝ₜ (λ i => if i < k then v₂ i else v₁ i) := by
+        simp [t]; ext i
+        rcases Nat.lt_trichotomy i k with (h | h | h)
+        · simp [h, Term.shift_subst_single]
+        · simp [h]; congr; apply Fin.eq_of_val_eq; simp [k', h]
+        · simp [Nat.not_lt_of_gt h, Nat.ne_of_gt h, Term.shift_subst_single]
+      have h₃ : t[↦ₛ (v₂ k')]ₜ = f ⬝ₜ (λ i => if i < k.succ then v₂ i else v₁ i) := by
+        simp [t]; ext i
+        rcases Nat.lt_trichotomy i k with (h | h | h)
+        · simp [h, Nat.lt_succ_of_lt h, Term.shift_subst_single]
+        · simp [h]; congr; apply Fin.eq_of_val_eq; simp [k', h]
+        · simp [Nat.not_lt_of_gt h, Nat.lt_succ, Nat.not_le_of_gt h,
+            Nat.ne_of_gt h, Term.shift_subst_single]
+      rw [←h₂, ←h₃]
+      papply subst_term
+      apply andN_elim (v := λ i => v₁ i ≐ v₂ i)
+      passumption
+
+theorem subst_term' :
+  (∀ i, Γ ⊢ σ₁ i ≐ σ₂ i) → Γ ⊢ t[σ₁]ₜ ≐ t[σ₂]ₜ := by
+  intro h
+  induction t with simp
+  | var => apply h
+  | func f v ih => papply congr_func; apply andN_intro; exact ih
+
+theorem congr_rel_iff {r} {v₁ v₂ : Vec 𝓛.Term n} :
+  Γ ⊢ (⋀i, v₁ i ≐ v₂ i) ⇒ r ⬝ᵣ v₁ ⇔ r ⬝ᵣ v₂ := by
+  pintro
+  suffices ∀ k ≤ n, _ ⊢ r ⬝ᵣ v₁ ⇔ r ⬝ᵣ (λ i => if i < k then v₂ i else v₁ i) by
+    replace this := this n (by rfl)
+    simp at this
+    exact this
+  intros k h₁
+  induction k with
+  | zero => simp; exact iff_refl
+  | succ k ih =>
+    papply iff_trans
+    · exact ih (Nat.le_of_succ_le h₁)
+    · let k' : Fin n := ⟨k, h₁⟩
+      let p := r ⬝ᵣ (λ i => if i < k then ↑ₜ(v₂ i) else if i = k then #0 else ↑ₜ(v₁ i))
+      have h₂ : p[↦ₛ (v₁ k')]ₚ = r ⬝ᵣ (λ i => if i < k then v₂ i else v₁ i) := by
+        simp [p]; ext i
+        rcases Nat.lt_trichotomy i k with (h | h | h)
+        · simp [h, Term.shift_subst_single]
+        · simp [h]; congr; apply Fin.eq_of_val_eq; simp [k', h]
+        · simp [Nat.not_lt_of_gt h, Nat.ne_of_gt h, Term.shift_subst_single]
+      have h₃ : p[↦ₛ (v₂ k')]ₚ = r ⬝ᵣ (λ i => if i < k.succ then v₂ i else v₁ i) := by
+        simp [p]; ext i
+        rcases Nat.lt_trichotomy i k with (h | h | h)
+        · simp [h, Nat.lt_succ_of_lt h, Term.shift_subst_single]
+        · simp [h]; congr; apply Fin.eq_of_val_eq; simp [k', h]
+        · simp [Nat.not_lt_of_gt h, Nat.lt_succ, Nat.not_le_of_gt h,
+            Nat.ne_of_gt h, Term.shift_subst_single]
+      rw [←h₂, ←h₃]
+      papply subst_iff
+      apply andN_elim (v := λ i => v₁ i ≐ v₂ i)
+      passumption
+
+theorem congr_rel {r} {v₁ v₂ : Vec 𝓛.Term n} :
+  Γ ⊢ (⋀i, v₁ i ≐ v₂ i) ⇒ r ⬝ᵣ v₁ ⇒ r ⬝ᵣ v₂ := by
+  pintro
+  papply iff_mp
+  papply congr_rel_iff
+  passumption
+
+theorem congr_eq : Γ ⊢ t₁ ≐ t₁' ⇒ t₂ ≐ t₂' ⇒ t₁ ≐ t₂ ⇒ t₁' ≐ t₂' := by
+  pintros
+  ptrans
+  · psymm; passumption
+  · ptrans <;> passumption
+
+theorem congr_eq_iff : Γ ⊢ t₁ ≐ t₁' ⇒ t₂ ≐ t₂' ⇒ t₁ ≐ t₂ ⇔ t₁' ≐ t₂' := by
+  pintros 2
+  papply iff_intro
+  · papply congr_eq <;> passumption
+  · papply congr_eq <;> psymm <;> passumption
+
+theorem subst_iff' : (∀ i, Γ ⊢ σ₁ i ≐ σ₂ i) → Γ ⊢ p[σ₁]ₚ ⇔ p[σ₂]ₚ := by
+  intro h
+  induction p generalizing Γ σ₁ σ₂ with simp
+  | rel r v =>
+    papply congr_rel_iff; apply andN_intro; intro; apply subst_term'; exact h
+  | eq t₁ t₂ =>
+    papply congr_eq_iff <;> apply subst_term' <;> exact h
+  | false =>
+    exact iff_refl
+  | imp p q ih₁ ih₂ =>
+    papply iff_congr_imp <;> apply_assumption <;> exact h
+  | all p ih =>
+    papply iff_congr_forall; apply generalization; apply ih; intro i
+    cases i with simp
+    | zero => prefl
+    | succ i => apply closed_under_shift (p := σ₁ i ≐ σ₂ i); apply h
+
+theorem subst' : (∀ i, Γ ⊢ σ₁ i ≐ σ₂ i) → Γ ⊢ p[σ₁]ₚ ⇒ p[σ₂]ₚ := by
+  intro h
+  papply iff_mp
+  exact subst_iff' h
+
+namespace Rewrite
+
+mutual
+inductive Term (Γ : 𝓛.Context) : 𝓛.Term → 𝓛.Term → Prop
+| matched {t₁ t₂} : Γ ⊢ t₁ ≐ t₂ → Term Γ t₁ t₂
+| func : Terms Γ v₁ v₂ → Term Γ (f ⬝ₜ v₁) (f ⬝ₜ v₂)
+| refl {t} : Term Γ t t
+inductive Terms (Γ : 𝓛.Context) : Vec 𝓛.Term n → Vec 𝓛.Term n → Prop
+| cons {t₁ t₂} : Term Γ t₁ t₂ → Terms Γ v₁ v₂ → Terms Γ (t₁ ∷ᵥ v₁) (t₂ ∷ᵥ v₂)
+| refl : Terms Γ v v
+end
+
+theorem Terms.term :
+  ∀ {n} {v₁ v₂ : Vec 𝓛.Term n}, Terms Γ v₁ v₂ → ∀ i, Term Γ (v₁ i) (v₂ i)
+| _, _, _, cons h₁ h₂, i => i.cases h₁ (λ _ => h₂.term _)
+| _, _, _, refl, _ => Term.refl
+
+theorem Term.sound : ∀ {t₁ t₂}, Term Γ t₁ t₂ → Γ ⊢ t₁ ≐ t₂
+| _, _, matched h => h
+| _, _, func h => by
+  papply congr_func; apply andN_intro; intro i; exact (h.term i).sound
+| _, _, refl => Proof.refl
+
+inductive Formula (Γ : 𝓛.Context) : 𝓛.Formula → 𝓛.Formula → Prop
+| rel {r v₁ v₂} : Terms Γ v₁ v₂ → Formula Γ (r ⬝ᵣ v₁) (r ⬝ᵣ v₂)
+| eq {t₁ t₁' t₂ t₂'} : Term Γ t₁ t₁' → Term Γ t₂ t₂' → Formula Γ (t₁ ≐ t₂) (t₁' ≐ t₂')
+| imp {p₁ q₁ p₂ q₂} : Formula Γ p₁ q₁ → Formula Γ p₂ q₂ → Formula Γ (p₁ ⇒ p₂) (q₁ ⇒ q₂)
+| refl {p} : Formula Γ p p
+
+theorem Formula.sound : Formula Γ p q → Γ ⊢ p ⇔ q := by
+  intro h
+  induction h with
+  | rel h => papply congr_rel_iff; apply andN_intro; intro i; exact (h.term i).sound
+  | eq => papply congr_eq_iff <;> apply Term.sound <;> assumption
+  | imp => papply iff_congr_imp <;> assumption
+  | refl => exact iff_refl
+
+macro "prewrite" t:term : tactic =>
+  `(tactic| (
+    apply mp2 iff_mpr
+    · apply Formula.sound
+      repeat' first
+      | apply Formula.rel | apply Formula.eq | apply Formula.imp | exact Formula.refl
+      | apply Terms.cons | exact Terms.refl
+      | exact Term.matched (by pexact $t) | apply Term.func | exact Term.refl
+    try simp))
+
+syntax rwRule := ("← "?) term
+
+/--
+  Rewrite goal using given terms.
+  If a number instead of term is given, it will use assumption in rewrite.
+  
+  Use `←` to change the direction. -/
+elab "prw" "[" rules:withoutPosition(rwRule,*,?) "]" : tactic => do
+  for rule in rules.raw.getSepArgs do
+    let t ←
+      match rule with
+      | `(rwRule | $n:num) => Lean.Elab.liftMacroM (hypTerm n.getNat)
+      | `(rwRule | $t:term) => pure t
+      | `(rwRule | ← $n:num) => `(mp symm $(← Lean.Elab.liftMacroM (hypTerm n.getNat)))
+      | `(rwRule | ← $t:term) => `(mp symm $t)
+      | _ => throwError "this shouldn't happen"
+    Lean.Elab.Tactic.evalTactic (←`(tactic| prewrite $t))
+
+end Rewrite
 
 theorem compactness : Γ ⊢ p → ∃ Δ, Δ ⊆ Γ ∧ Δ.Finite ∧ Δ ⊢ p := by
   intro h
   induction h with
-  | @assumption p h =>
-    exists {p}
-    constructor
-    · simp [h]
-    constructor
-    · simp
-    · passumption; rfl
-  | axioms h =>
-    exists ∅
-    constructor
-    · simp
-    constructor
-    · simp
-    · exact axioms h
+  | @hyp p h =>
+    exists {p}; simp [h]
+    passumption; rfl
+  | ax h =>
+    exists ∅; simp
+    exact ax h
   | mp _ _ ih₁ ih₂ =>
     rcases ih₁ with ⟨Δ₁, h₁, h₂, h₃⟩
     rcases ih₂ with ⟨Δ₂, h₄, h₅, h₆⟩
-    exists Δ₁ ∪ Δ₂
-    constructor
-    · simp [h₁, h₄]
-    constructor
-    · simp [h₂, h₅]
-    · apply Proof.mp
-      · apply weaken
-        · apply Set.subset_union_left
-        · exact h₃
-      · apply weaken
-        · apply Set.subset_union_right
-        · exact h₆
+    exists Δ₁ ∪ Δ₂; simp [h₁, h₄, h₂, h₅]
+    apply Proof.mp
+    · apply weaken _ h₃; simp
+    · apply weaken _ h₆; simp
 
 end Proof
 
-
-
 notation Γ:50 "⊬" p:50 => ¬ Γ ⊢ p
 
-def Consistent (Γ : Context 𝓛) := Γ ⊬ ⊥
+namespace Context
+
+def Consistent (Γ : 𝓛.Context) := Γ ⊬ ⊥
 
 theorem Consistent.weaken : Γ ⊆ Δ → Consistent Δ → Consistent Γ := by
   intros h₁ h₂ h
   apply h₂
-  apply Proof.weaken
-  · exact h₁
-  · exact h
+  exact Proof.weaken h₁ h
 
-theorem Consistent.add : Consistent (Γ,' p) ↔ Γ ⊬ ~ p := by
+theorem Consistent.append : Consistent (Γ,, p) ↔ Γ ⊬ ~ p := by
   constructor
   · intro h₁ h₂
     apply h₁
@@ -364,3 +699,5 @@ theorem Consistent.add : Consistent (Γ,' p) ↔ Γ ⊬ ~ p := by
     apply h₁
     pintro
     exact h₂
+
+end Language.Context
