MathematicalLogic/FirstOrder/Syntax.lean
@@ -1,369 +1,263 @@
-import Mathlib.Data.Nat.Basic
-import Mathlib.Data.Set.Lattice
+import MathematicalLogic.Vector
 import MathematicalLogic.Notation
+import Mathlib.Data.Set.Lattice
+
+namespace FirstOrder
 
 structure Language where
   𝓕 : ℕ → Type
-  𝓟 : ℕ → Type
+  [decEq𝓕 : ∀ {n}, DecidableEq (𝓕 n)]
+  𝓡 : ℕ → Type
+  [decEq𝓡 : ∀ {n}, DecidableEq (𝓡 n)]
+
+namespace Language
 
 variable {𝓛 : Language}
-abbrev Const (𝓛 : Language) := 𝓛.𝓕 0
 
-mutual
+abbrev Const := 𝓛.𝓕 0
+instance : DecidableEq (𝓛.𝓕 n) := 𝓛.decEq𝓕
+instance : DecidableEq (𝓛.𝓡 n) := 𝓛.decEq𝓡
+
 inductive Term (𝓛 : Language) : Type where
-| var : ℕ → Term 𝓛
-| func : 𝓛.𝓕 n → Terms 𝓛 n → Term 𝓛
-inductive Terms (𝓛 : Language) : ℕ → Type where
-| nil : Terms 𝓛 0
-| cons : Term 𝓛 → Terms 𝓛 n → Terms 𝓛 (n + 1)
-end
-
+| var : ℕ → 𝓛.Term
+| func : 𝓛.𝓕 n → (Fin n → 𝓛.Term) → 𝓛.Term
 prefix:max "#" => Term.var
 infix:70 " ⬝ₜ " => Term.func
-notation "[]ₜ" => Terms.nil
-infixr:75 " ∷ₜ " => Terms.cons
+instance : Coe 𝓛.Const 𝓛.Term := ⟨λ c => c ⬝ₜ []ᵥ⟩
 
-instance : Coe (Const 𝓛) (Term 𝓛) where
-  coe := λ c => c ⬝ₜ []ₜ
+instance Term.decEq : DecidableEq 𝓛.Term := by
+  intro t₁ t₂
+  cases t₁ <;> cases t₂
+  case var.var => rw [Term.var.injEq]; apply Nat.decEq
+  case func.func n f v₁ m g v₂ =>
+    by_cases h : n = m
+    · subst h; simp [Term.func.injEq]; rw [←Vec.ext_iff]
+      have := λ i => decEq (v₁ i) (v₂ i)
+      apply And.decidable
+    · simp [h]; exact isFalse not_false
+  all_goals exact isFalse Term.noConfusion
 
-def Terms.ofVector : Vector (Term 𝓛) n → Terms 𝓛 n
-| ⟨l, h⟩ =>
-  match n, l with
-  | 0, [] => []ₜ
-  | n + 1, t :: l => t ∷ₜ Terms.ofVector ⟨l, by simp at h; exact h⟩
-
-@[simp] lemma Terms.of_vector_nil : Terms.ofVector []ᵥ = ([]ₜ : Terms 𝓛 0) := rfl
-@[simp] lemma Terms.of_vector_cons : Terms.ofVector (t ∷ᵥ v) = t ∷ₜ Terms.ofVector v := rfl
-
-instance : Coe (Vector (Term 𝓛) n) (Terms 𝓛 n) where
-  coe := Terms.ofVector
-
-mutual
-@[simp] def Term.size : Term 𝓛 → ℕ
-| #_ => 0
-| _ ⬝ₜ ts => ts.size + 1
-@[simp] def Terms.size : Terms 𝓛 n → ℕ
-| []ₜ => 0
-| t ∷ₜ ts => t.size + ts.size + 1
-end
-
-instance (priority := high) : SizeOf (Term 𝓛) := ⟨Term.size⟩
-instance (priority := high) : SizeOf (Terms 𝓛 n) := ⟨Terms.size⟩
-@[simp] theorem Term.sizeOf_eq {t : Term 𝓛} : sizeOf t = t.size := rfl
-@[simp] theorem Terms.sizeOf_eq {ts : Terms 𝓛 n} : sizeOf ts = ts.size := rfl
-
-mutual
-def Term.vars : Term 𝓛 → Set ℕ
+def Term.vars : 𝓛.Term → Set ℕ
 | #x => {x}
-| _ ⬝ₜ ts => ts.vars
-def Terms.vars : Terms 𝓛 n → Set ℕ
-| []ₜ => {}
-| t ∷ₜ ts => t.vars ∪ ts.vars
-end
+| _ ⬝ₜ v => ⋃ i, (v i).vars
 
-def Terms.append : Terms 𝓛 n → Terms 𝓛 m → Terms 𝓛 (m + n)
-| []ₜ, ts => ts
-| t ∷ₜ ts, ts' => t ∷ₜ ts.append ts'
+def Subst (𝓛 : Language) := ℕ → 𝓛.Term
 
-instance : HAppend (Terms 𝓛 n) (Terms 𝓛 m) (Terms 𝓛 (m + n)) := ⟨Terms.append⟩
-
-@[simp] theorem Terms.nil_append {ts : Terms 𝓛 n} : ([]ₜ : Terms 𝓛 0) ++ ts = ts := rfl
-@[simp] theorem Terms.cons_append {ts : Terms 𝓛 n} {ts' : Terms 𝓛 m} : t ∷ₜ ts ++ ts' = t ∷ₜ (ts ++ ts') := rfl
-
-theorem Terms.append_nil {ts : Terms 𝓛 n} :
-  HEq (ts ++ ([]ₜ : Terms 𝓛 0)) ts :=
-  match ts with
-  | []ₜ => by simp
-  | t ∷ₜ ts => by
-    simp; congr
-    · simp
-    · apply Terms.append_nil
-
-theorem Terms.append_assoc {ts₁ : Terms 𝓛 n} {ts₂ : Terms 𝓛 m} {ts₃ : Terms 𝓛 k} :
-  HEq (ts₁ ++ (ts₂ ++ ts₃)) (ts₁ ++ ts₂ ++ ts₃) :=
-  match ts₁ with
-  | []ₜ => by simp
-  | t ∷ₜ ts => by
-    simp; congr 1
-    · simp [Nat.add_assoc]
-    · apply Terms.append_assoc
-
-theorem Terms.append_cons {ts₁ : Terms 𝓛 n} {ts₂ : Terms 𝓛 m} :
-  HEq (ts₁ ++ t₁ ∷ₜ ts₂) ((ts₁ ++ t₁ ∷ₜ []ₜ) ++ ts₂) := by
-  conv in t₁ ∷ₜ ts₂ =>
-    rw [←Terms.nil_append (ts := ts₂), ←Terms.cons_append]
-  apply Terms.append_assoc
-
-
-
-def Subst (𝓛) := ℕ → Term 𝓛
-
-mutual
-def Term.subst : Term 𝓛 → Subst 𝓛 → Term 𝓛
+def Term.subst : 𝓛.Term → 𝓛.Subst → 𝓛.Term
 | #x, σ => σ x
-| f ⬝ₜ ts, σ => f ⬝ₜ (ts.subst σ)
-def Terms.subst : Terms 𝓛 n → Subst 𝓛 → Terms 𝓛 n
-| []ₜ, _ => []ₜ
-| t ∷ₜ ts, σ => t.subst σ ∷ₜ ts.subst σ
-end
-
+| f ⬝ₜ v, σ => f ⬝ₜ λ i => (v i).subst σ
 notation:80 t "[" σ "]ₜ" => Term.subst t σ
-notation:80 ts "[" σ "]ₜₛ" => Terms.subst ts σ
+@[simp] theorem Term.subst_var : (#x)[σ]ₜ = σ x := rfl
+@[simp] theorem Term.subst_func : (f ⬝ₜ v)[σ]ₜ = f ⬝ₜ λ i => (v i)[σ]ₜ := rfl
 
-@[simp] theorem Term.subst_var : (#x)[σ]ₜ = σ x := by simp [Term.subst]
-@[simp] theorem Term.subst_func : (f ⬝ₜ ts)[σ]ₜ = f ⬝ₜ ts[σ]ₜₛ := by simp [Term.subst]
-@[simp] theorem Terms.subst_nil : []ₜ[σ]ₜₛ = []ₜ := rfl
-@[simp] theorem Terms.subst_cons : (t ∷ₜ ts)[σ]ₜₛ = t[σ]ₜ ∷ₜ ts[σ]ₜₛ := by simp [Terms.subst]
+def Subst.id : 𝓛.Subst := (#·)
+@[simp] theorem Subst.id_app : (id x : 𝓛.Term) = #x := rfl
+@[simp] theorem Term.subst_id : t[Subst.id]ₜ = t := by
+  induction t with simp
+  | func f v ih => ext; apply ih
 
-theorem Terms.subst_append : (ts₁ ++ ts₂)[σ]ₜₛ = ts₁[σ]ₜₛ ++ ts₂[σ]ₜₛ :=
-  match ts₁ with
-  | []ₜ => rfl
-  | t ∷ₜ ts => by simp [Terms.subst]; apply Terms.subst_append
-
-def Subst.id : Subst 𝓛 := λ x => #x
-notation "idₛ" => Subst.id
-
-@[simp] theorem Subst.id_app : (idₛ x : Term 𝓛) = #x := rfl
-
-mutual
-theorem Term.subst_id : t[idₛ]ₜ = t :=
-  match t with
-  | #x => by simp
-  | f ⬝ₜ ts => by simp; rw [Terms.subst_id]
-theorem Terms.subst_id : ts[idₛ]ₜₛ = ts :=
-  match ts with
-  | []ₜ => by rfl
-  | t ∷ₜ ts => by simp; rw [Term.subst_id, Terms.subst_id]; trivial
-end
-
-def Subst.comp (σ₁ σ₂ : Subst 𝓛) : Subst 𝓛 := λ x => (σ₁ x)[σ₂]ₜ
+def Subst.comp (σ₁ σ₂ : 𝓛.Subst) : 𝓛.Subst := λ x => (σ₁ x)[σ₂]ₜ
 infixl:90 " ∘ₛ " => Subst.comp
-@[simp] theorem Subst.comp_app {σ₁ σ₂ : Subst 𝓛} : (σ₁ ∘ₛ σ₂) x = (σ₁ x)[σ₂]ₜ := rfl
+@[simp] theorem Subst.comp_app : (σ₁ ∘ₛ σ₂) x = (σ₁ x)[σ₂]ₜ := rfl
+@[simp] theorem Term.subst_comp : t[σ₁ ∘ₛ σ₂]ₜ = t[σ₁]ₜ[σ₂]ₜ := by
+  induction t with simp
+  | func f v ih => ext; apply ih
 
-mutual
-theorem Term.subst_comp : t[σ₁]ₜ[σ₂]ₜ = t[σ₁ ∘ₛ σ₂]ₜ :=
-  match t with
-  | #x => by simp
-  | f ⬝ₜ ts => by simp; rw [Terms.subst_comp]
-theorem Terms.subst_comp : ts[σ₁]ₜₛ[σ₂]ₜₛ = ts[σ₁ ∘ₛ σ₂]ₜₛ :=
-  match ts with
-  | []ₜ => by rfl
-  | t ∷ₜ ts => by simp; rw [Term.subst_comp, Terms.subst_comp]; trivial
-end
-
-def Subst.cons (t : Term 𝓛) (σ : Subst 𝓛) : Subst 𝓛
+def Subst.cons (t : 𝓛.Term) (σ : 𝓛.Subst) : 𝓛.Subst
 | 0 => t
 | x + 1 => σ x
-infix:90 " ∷ₛ " => Subst.cons
+infixl:90 " ∷ₛ " => Subst.cons
 @[simp] theorem Subst.cons_app_zero : (t ∷ₛ σ) 0 = t := rfl
 @[simp] theorem Subst.cons_app_succ : (t ∷ₛ σ) (x + 1) = σ x := rfl
 
-def Subst.single : Term 𝓛 → Subst 𝓛
-| t, 0 => t
-| _, x + 1 => #x
+def Subst.single (t : 𝓛.Term) : 𝓛.Subst := t ∷ₛ id
 prefix:max "↦ₛ " => Subst.single
 @[simp] theorem Subst.single_app_zero : (↦ₛ t) 0 = t := rfl
 @[simp] theorem Subst.single_app_succ : (↦ₛ t) (x + 1) = #x := rfl
 
-def Subst.shift : Subst 𝓛 := λ x => #(x + 1)
-@[simp] theorem Subst.shift_app : (Subst.shift x : Term 𝓛) = #(x + 1) := rfl
-
-def Term.shift (t : Term 𝓛) := t[Subst.shift]ₜ
+def Subst.shift : 𝓛.Subst := λ x => #(x + 1)
+def Term.shift (t : 𝓛.Term) := t[Subst.shift]ₜ
 prefix:max "↑ₜ" => Term.shift
-@[simp] theorem Term.shift_var : ↑ₜ(#x : Term 𝓛) = #(x + 1) := by simp [Term.shift, Subst.shift]
-
-def Terms.shift (ts : Terms 𝓛 n) := ts[Subst.shift]ₜₛ
-prefix:max "↑ₜₛ" => Terms.shift
-
-lemma Subst.shift_comp_single : Subst.shift ∘ₛ ↦ₛ t = idₛ := rfl
-
-theorem Term.shift_subst_single : (↑ₜt₁)[↦ₛ t₂]ₜ = t₁ := by
-  rw [Term.shift, Term.subst_comp, Subst.shift_comp_single, Term.subst_id]
-
-theorem Terms.shift_subst_single : (↑ₜₛts)[↦ₛ t]ₜₛ = ts := by
-  rw [Terms.shift, Terms.subst_comp, Subst.shift_comp_single, Terms.subst_id]
+@[simp] theorem Subst.shift_app : (shift x : 𝓛.Term) = #(x + 1) := rfl
+@[simp] theorem Term.shift_var : ↑ₜ(#x : 𝓛.Term) = #(x + 1) := rfl
 
 theorem Term.shift_subst_cons : (↑ₜt₁)[t₂ ∷ₛ σ]ₜ = t₁[σ]ₜ := by
-  rw [Term.shift, Term.subst_comp]; rfl
+  rw [shift, ←subst_comp]; rfl
+theorem Term.shift_subst_single : (↑ₜt₁)[↦ₛ t₂]ₜ = t₁ := by
+  simp [Subst.single]; rw [shift_subst_cons, subst_id]
 
-def Subst.lift : Subst 𝓛 → Subst 𝓛
-| _, 0 => #0
-| σ, x + 1 => ↑ₜ(σ x)
+def Subst.assign (t : 𝓛.Term) : 𝓛.Subst := t ∷ₛ shift
+prefix:max "≔ₛ " => Subst.assign
+@[simp] theorem Subst.assign_app_zero : (≔ₛ t) 0 = t := rfl
+@[simp] theorem Subst.assign_app_succ : (≔ₛ t) (x + 1) = #(x + 1) := rfl
+
+def Subst.lift (σ : 𝓛.Subst) : 𝓛.Subst
+| 0 => #0
+| x + 1 => ↑ₜ(σ x)
 prefix:max "⇑ₛ" => Subst.lift
 @[simp] theorem Subst.lift_app_zero : ⇑ₛσ 0 = #0 := rfl
 @[simp] theorem Subst.lift_app_succ : ⇑ₛσ (x + 1) = ↑ₜ(σ x) := rfl
-
 theorem Term.shift_subst_lift : (↑ₜt)[⇑ₛσ]ₜ = ↑ₜ(t[σ]ₜ) := by
-  rw [Term.shift, Term.shift, Term.subst_comp, Term.subst_comp]
-  congr
-
-theorem Subst.lift_id : ⇑ₛ(idₛ : Subst 𝓛) = idₛ := by
-  funext x
-  cases x <;> simp
-
+  simp_rw [shift, ←subst_comp]; congr
+theorem Subst.lift_id : ⇑ₛ(@id 𝓛) = id := by
+  funext x; cases x <;> simp
 theorem Subst.lift_comp : ⇑ₛ(σ₁ ∘ₛ σ₂) = ⇑ₛσ₁ ∘ₛ ⇑ₛσ₂ := by
-  funext x
-  cases x with
-  | zero => rfl
-  | succ =>
-    simp [Subst.comp, Term.subst, Term.shift_subst_lift]
+  funext x; cases x <;> simp [Term.shift_subst_lift]
 
-mutual
-theorem Term.subst_ext_vars {t : Term 𝓛} :
-  (∀ x ∈ t.vars, σ₁ x = σ₂ x) → t[σ₁]ₜ = t[σ₂]ₜ :=
-  match t with
-  | #x => by intro h; simp [h, Term.vars]
-  | f ⬝ₜ ts => by
-    intro h
-    simp [Term.vars] at h
-    simp
-    apply Terms.subst_ext_vars
-    exact h
-theorem Terms.subst_ext_vars {ts : Terms 𝓛 n} :
-  (∀ x ∈ ts.vars, σ₁ x = σ₂ x) → ts[σ₁]ₜₛ = ts[σ₂]ₜₛ :=
-  match ts with
-  | []ₜ => by intro; rfl
-  | t ∷ₜ ts => by
-    intro h
-    simp [Terms.vars] at h
-    simp
-    constructor
-    · apply Term.subst_ext_vars; intros; apply h; left; assumption
-    · apply Terms.subst_ext_vars; intros; apply h; right; assumption
-end
+theorem Term.subst_ext_vars {t : 𝓛.Term} (h : ∀ x ∈ t.vars, σ₁ x = σ₂ x) :
+  t[σ₁]ₜ = t[σ₂]ₜ := by
+  induction t with simp [h, vars]
+  | func t v ih => ext i; apply ih; intros; apply h; simp [vars]; exists i
 
-mutual
-theorem Term.vars_of_subst : t[σ]ₜ.vars = ⋃ x ∈ t.vars, (σ x).vars :=
-  match t with
-  | #x => by simp [Term.vars]
-  | f ⬝ₜ ts => by simp [Term.vars]; rw [Terms.vars_of_subst]
-theorem Terms.vars_of_subst : ts[σ]ₜₛ.vars = ⋃ x ∈ ts.vars, (σ x).vars :=
-  match ts with
-  | []ₜ => by simp [Terms.vars]
-  | t ∷ₜ ts => by
-    conv => lhs; simp [Terms.vars]
-    conv => rhs; rw [Terms.vars]
-    rw [Term.vars_of_subst, Terms.vars_of_subst, Set.biUnion_union]
-end
+theorem Term.vars_of_subst : t[σ]ₜ.vars = ⋃ x ∈ t.vars, (σ x).vars := by
+  induction t with simp [vars]
+  | func t v ih => rw [Set.iUnion_comm]; simp_rw [ih]
 
 theorem Term.is_shift_iff : (∃ t', t = ↑ₜt') ↔ 0 ∉ t.vars := by
   constructor
-  · rintro ⟨t, h⟩
-    subst h
-    intro h
-    simp [Term.shift, Term.vars_of_subst] at h
+  · rintro ⟨t, h⟩; subst h
+    intro h; simp [shift, vars_of_subst] at h
     rcases h with ⟨x, ⟨_, h⟩⟩
     contradiction
   · intro h
     exists t[↦ₛ #0]ₜ
-    rw [Term.shift, Term.subst_comp]
-    conv => lhs; rw [←Term.subst_id (t := t)]
-    apply Term.subst_ext_vars
+    rw [shift, ←subst_comp]
+    conv => lhs; rw [←subst_id (t := t)]
+    apply subst_ext_vars
     intros x h₁
     cases x
     · contradiction
-    · simp [Subst.id, Subst.comp, Subst.shift, Subst.single]
+    · rfl
+
+theorem Term.subst_swap : t[↦ₛ t₁]ₜ[σ]ₜ = t[⇑ₛσ]ₜ[↦ₛ (t₁[σ]ₜ)]ₜ := by
+  simp_rw [←subst_comp]
+  congr; funext i
+  cases i <;> simp [shift_subst_single]
 
 
 
 inductive Formula (𝓛 : Language) : Type where
-| atom : 𝓛.𝓟 n → Terms 𝓛 n → Formula 𝓛
-| fal : Formula 𝓛
-| imp : Formula 𝓛 → Formula 𝓛 → Formula 𝓛
-| all : Formula 𝓛 → Formula 𝓛
-
-infix:70 " ⬝ₚ " => Formula.atom
-instance : FormulaSymbol (Formula 𝓛) := ⟨Formula.fal, Formula.imp⟩
+| rel : 𝓛.𝓡 n → (Fin n → 𝓛.Term) → 𝓛.Formula
+| eq : 𝓛.Term → 𝓛.Term → 𝓛.Formula
+| false : 𝓛.Formula
+| imp : 𝓛.Formula → 𝓛.Formula → 𝓛.Formula
+| all : 𝓛.Formula → 𝓛.Formula
+infix:70 " ⬝ᵣ " => Formula.rel
+instance : PropNotation 𝓛.Formula := ⟨Formula.false, Formula.imp⟩
 prefix:59 "∀' " => Formula.all
-abbrev Formula.exists (p : Formula 𝓛) := ~ ∀' (~ p)
-prefix:59 "∃' " => Formula.exists
+abbrev Formula.exist (p : 𝓛.Formula) := ~ ∀' (~ p)
+prefix:59 "∃' " => Formula.exist
 
-@[simp] theorem Formula.fal_eq : Formula.fal = (⊥ : Formula 𝓛) := rfl
+def Formula.andN : {n : ℕ} → Vec 𝓛.Formula n → 𝓛.Formula
+| 0, _ => ⊤
+| _ + 1, v => v.head ⩑ andN v.tail
+notation3:57 "⋀"(...)", " r:(scoped r => Formula.andN r) => r
+
+infix:60 (priority := high) " ≐ " => Formula.eq
+
+@[simp] theorem Formula.false_eq : Formula.false = (⊥ : 𝓛.Formula) := rfl
 @[simp] theorem Formula.imp_eq : Formula.imp p q = p ⇒ q := rfl
 
-def Formula.free : Formula 𝓛 → Set ℕ
-| _ ⬝ₚ ts => ts.vars
+instance Formula.decEq : DecidableEq 𝓛.Formula := by
+  intro p q
+  cases p <;> cases q
+  case rel.rel n r₁ v₁ m r₂ v₂ =>
+    by_cases h : n = m
+    · subst h; simp [Formula.rel.injEq]; rw [←Vec.ext_iff]
+      apply And.decidable
+    · simp [h]; exact isFalse not_false
+  case eq.eq =>
+    rw [Formula.eq.injEq]; apply And.decidable
+  case false.false => exact isTrue rfl
+  case imp.imp p₁ q₁ p₂ q₂ =>
+    rw [Formula.imp.injEq]
+    have := decEq p₁ p₂
+    have := decEq q₁ q₂
+    apply And.decidable
+  case all.all p q =>
+    rw [Formula.all.injEq]
+    exact decEq p q
+  all_goals exact isFalse Formula.noConfusion
+
+def Formula.free : 𝓛.Formula → Set ℕ
+| _ ⬝ᵣ ts => ⋃ i, (ts i).vars
+| t₁ ≐ t₂ => t₁.vars ∪ t₂.vars
 | ⊥ => {}
 | p ⇒ q => p.free ∪ q.free
 | ∀' p => { x | x + 1 ∈ p.free }
 
-def Formula.subst : Formula 𝓛 → Subst 𝓛 → Formula 𝓛
-| p ⬝ₚ ts, σ => p ⬝ₚ ts[σ]ₜₛ
+def Formula.subst : 𝓛.Formula → 𝓛.Subst → 𝓛.Formula
+| r ⬝ᵣ ts, σ => r ⬝ᵣ (λ i => (ts i).subst σ)
+| t₁ ≐ t₂, σ => t₁.subst σ ≐ t₂.subst σ
 | ⊥, _ => ⊥
 | p ⇒ q, σ => p.subst σ ⇒ q.subst σ
 | ∀' p, σ => ∀' (p.subst ⇑ₛσ)
-
 notation:80 p "[" σ "]ₚ" => Formula.subst p σ
-
-@[simp] theorem Formula.subst_atom : (p ⬝ₚ ts)[σ]ₚ = p ⬝ₚ ts[σ]ₜₛ := rfl
-@[simp] theorem Formula.subst_fal : ⊥[σ]ₚ = ⊥ := rfl
+@[simp] theorem Formula.subst_rel : (r ⬝ᵣ ts)[σ]ₚ = r ⬝ᵣ (λ i => (ts i)[σ]ₜ) := rfl
+@[simp] theorem Formula.subst_eq : (t₁ ≐ t₂)[σ]ₚ = t₁[σ]ₜ ≐ t₂[σ]ₜ := rfl
+@[simp] theorem Formula.subst_false : ⊥[σ]ₚ = ⊥ := rfl
 @[simp] theorem Formula.subst_imp : (p ⇒ q)[σ]ₚ = p[σ]ₚ ⇒ q[σ]ₚ := rfl
+@[simp] theorem Formula.subst_all : (∀' p)[σ]ₚ = ∀' (p[⇑ₛσ]ₚ) := rfl
 @[simp] theorem Formula.subst_neg : (~ p)[σ]ₚ = ~ p[σ]ₚ := rfl
-@[simp] theorem Formula.subst_all : (∀' p)[σ]ₚ = ∀' p[⇑ₛσ]ₚ := rfl
 
-def Formula.shift : Formula 𝓛 → Formula 𝓛 := λ p => p[Subst.shift]ₚ
+def Formula.shift : 𝓛.Formula → 𝓛.Formula := λ p => p[Subst.shift]ₚ
 prefix:max "↑ₚ" => Formula.shift
 
-theorem Formula.subst_ext : σ₁ = σ₂ → p[σ₁]ₚ = p[σ₂]ₚ := by intro h; rw [h]
+abbrev Formula.existUnique (p : 𝓛.Formula) :=
+  ∃' (p ⩑ ∀' ((↑ₚp)[≔ₛ #0]ₚ ⇒ #0 ≐ #1))
+prefix:59 "∃!' " => Formula.existUnique
 
-theorem Formula.subst_id : p[idₛ]ₚ = p := by
-  induction p with
-  | atom => simp [Terms.subst_id]
-  | fal => rfl
-  | imp _ _ ih₁ ih₂ => simp [ih₁, ih₂]
-  | all _ ih => simp [Subst.lift_id, ih]
+theorem Formula.subst_id : p[Subst.id]ₚ = p := by
+  induction p with simp
+  | imp p q ih₁ ih₂ => simp [ih₁, ih₂]
+  | all p ih => simp [Subst.lift_id, ih]
 
-theorem Formula.subst_comp : p[σ₁]ₚ[σ₂]ₚ = p[σ₁ ∘ₛ σ₂]ₚ := by
-  induction p generalizing σ₁ σ₂ with
-  | atom => simp [Terms.subst_comp]
-  | fal => rfl
-  | imp _ _ ih₁ ih₂ => simp [ih₁, ih₂]
-  | all _ ih => simp [Subst.lift_comp, ih]
+theorem Formula.subst_comp : p[σ₁ ∘ₛ σ₂]ₚ = p[σ₁]ₚ[σ₂]ₚ := by
+  induction p generalizing σ₁ σ₂ with simp
+  | imp p q ih₁ ih₂ => simp [ih₁, ih₂]
+  | all p ih => simp [Subst.lift_comp, ih]
 
 theorem Formula.shift_subst_single : (↑ₚp)[↦ₛ t₂]ₚ = p := by
-  rw [Formula.shift, Formula.subst_comp]
-  conv => rhs; rw [←Formula.subst_id (p := p)]
+  rw [shift, ←subst_comp]
+  conv => rhs; rw [←subst_id (p := p)]
 
-theorem Formula.subst_ext_free {p : Formula 𝓛} :
+theorem Formula.shift_subst_lift : (↑ₚp)[⇑ₛσ]ₚ = ↑ₚ(p[σ]ₚ) := by
+  simp_rw [shift, ←subst_comp]; congr
+
+theorem Formula.subst_ext_free {p : 𝓛.Formula} :
   (∀ x ∈ p.free, σ₁ x = σ₂ x) → p[σ₁]ₚ = p[σ₂]ₚ := by
   intro h
-  induction p generalizing σ₁ σ₂ with
-  | atom =>
-    simp [Formula.free] at h
-    simp [Terms.subst_ext_vars h]
-  | fal => rfl
-  | imp _ _ ih₁ ih₂ =>
-    simp at h; simp; rw [ih₁, ih₂]
-    · intros; apply h; right; assumption
-    · intros; apply h; left; assumption
-  | all _ ih =>
-    simp [Formula.free] at h
-    simp; rw [ih]
-    intros x h₁
-    cases x
-    · rfl
-    · simp [Subst.lift]; congr; apply h; exact h₁
-
-theorem Formula.free_of_subst : p[σ]ₚ.free = ⋃ x ∈ p.free, (σ x).vars := by
-  induction p generalizing σ with
-  | atom => simp [Formula.free, Terms.vars_of_subst]
-  | fal => simp [Formula.free]
+  induction p generalizing σ₁ σ₂ with simp
+  | rel =>
+    ext i; apply Term.subst_ext_vars
+    intros; apply h; simp [free]
+    exists i
+  | eq =>
+    constructor <;> apply Term.subst_ext_vars
+      <;> intros _ h₁ <;> apply h <;> simp [free, h₁]
   | imp p q ih₁ ih₂ =>
-    conv => lhs; simp [Formula.free]
-    conv => rhs; rw [Formula.free]
-    rw [ih₁, ih₂, Set.biUnion_union]
+    congr 1 <;> apply_assumption
+      <;> intros _ h₁ <;> apply h <;> simp [free, h₁]
+  | all _ ih =>
+    apply ih; intro x h₁; cases x <;> simp
+    · congr; apply h; simp [free]; exact h₁
+
+theorem Formula.free_of_subst :
+  p[σ]ₚ.free = ⋃ x ∈ p.free, (σ x).vars := by
+  induction p generalizing σ with simp_rw [Formula.free]
+  | rel => simp [Term.vars_of_subst]; rw [Set.iUnion_comm]
+  | eq => simp [Set.iUnion_or, Set.iUnion_union_distrib, Term.vars_of_subst]
+  | false => simp
+  | imp p q ih₁ ih₂ => rw [ih₁, ih₂, Set.biUnion_union]
   | all p ih =>
-    conv => lhs; simp [Formula.free, ih]
-    conv => rhs; rw [Formula.free]
-    apply Set.ext
-    intro x; simp
+    ext x; simp [ih]
     constructor
-    · rintro ⟨y, ⟨h₁, h₂⟩⟩
+    · rintro ⟨y, h₁, h₂⟩
       cases y with
       | zero => contradiction
       | succ y =>
         simp [Subst.lift, Term.shift, Term.vars_of_subst] at h₂
-        rcases h₂ with ⟨z, ⟨h₂, h₃⟩⟩
+        rcases h₂ with ⟨z, h₂, h₃⟩
         simp [Subst.shift, Term.vars] at h₃
         subst h₃
         exists y
@@ -379,15 +273,224 @@ theorem Formula.is_shift_iff : (∃ p', p = ↑ₚp') ↔ 0 ∉ p.free := by
   · rintro ⟨p', h⟩
     subst h
     intro h
-    simp [Formula.shift, Formula.free_of_subst] at h
+    simp [shift, free_of_subst] at h
     rcases h with ⟨x, ⟨_, h⟩⟩
     contradiction
   · intro h
     exists p[↦ₛ #0]ₚ
-    rw [Formula.shift, Formula.subst_comp]
-    conv => lhs; rw [←Formula.subst_id (p := p)]
-    apply Formula.subst_ext_free
+    rw [shift, ←subst_comp]
+    conv => lhs; rw [←subst_id (p := p)]
+    apply subst_ext_free
     intros x h₁
     cases x
     · contradiction
-    · simp [Subst.id, Subst.comp, Subst.shift, Subst.single]
+    · rfl
+
+theorem Formula.subst_swap : p[↦ₛ t]ₚ[σ]ₚ = p[⇑ₛσ]ₚ[↦ₛ (t[σ]ₜ)]ₚ := by
+  simp_rw [←subst_comp]
+  congr; funext i
+  cases i <;> simp [Term.shift_subst_single]
+
+
+
+inductive BTerm (𝓛 : Language) : ℕ → Type where
+| var : Fin n → 𝓛.BTerm n
+| func : 𝓛.𝓕 m → (Fin m → 𝓛.BTerm n) → 𝓛.BTerm n
+prefix:max "#ᵇ" => BTerm.var
+infix:70 " ⬝ₜᵇ " => BTerm.func
+instance : Coe 𝓛.Const (𝓛.BTerm n) := ⟨λ c => c ⬝ₜᵇ []ᵥ⟩
+
+def BTerm.val : 𝓛.BTerm m → 𝓛.Term
+| #ᵇx => #x
+| f ⬝ₜᵇ v => f ⬝ₜ λ i => (v i).val
+@[simp] theorem BTerm.val_var : (#ᵇx : 𝓛.BTerm m).val = #x := rfl
+@[simp] theorem BTerm.val_func : (f ⬝ₜᵇ v).val = f ⬝ₜ λ i => (v i).val := rfl
+
+@[simp] def Term.bound : 𝓛.Term → ℕ
+| #x => x + 1
+| _ ⬝ₜ v => Vec.max (λ i => (v i).bound)
+
+theorem BTerm.property : (t : 𝓛.BTerm m).val.bound ≤ m := by
+  induction t with simp
+  | var x => exact x.isLt
+  | func f v ih => apply Vec.max_le; intro; apply ih
+
+def BTerm.mk :
+  (t : 𝓛.Term) → m ≥ t.bound → 𝓛.BTerm m
+| #x, h => #ᵇ⟨x, by simp at h; exact h⟩
+| f ⬝ₜ v, h => f ⬝ₜᵇ (λ i => mk (v i) (Nat.le_trans (Vec.le_max (v := Term.bound ∘ v)) h))
+
+theorem BTerm.val_mk {t : 𝓛.Term} {h : m ≥ t.bound} :
+  (mk t h).val = t := by
+  induction t with simp [mk]
+  | func f ts ih => ext; simp [ih]
+
+def BSubst (𝓛 : Language) (n m) := Vec (𝓛.BTerm m) n
+
+def BTerm.subst : 𝓛.BTerm n → 𝓛.BSubst n m → 𝓛.BTerm m
+| #ᵇ x, σ => σ x
+| f ⬝ₜᵇ v, σ => f ⬝ₜᵇ (λ i => (v i).subst σ)
+notation:80 t "[" σ "]ₜᵇ" => BTerm.subst t σ
+
+@[simp] theorem BTerm.subst_var : (#ᵇx)[σ]ₜᵇ = σ x := rfl
+@[simp] theorem BTerm.subst_func : (f ⬝ₜᵇ v)[σ]ₜᵇ = f ⬝ₜᵇ (λ i => (v i)[σ]ₜᵇ) := rfl
+
+def BSubst.id : 𝓛.BSubst n n := λ i => #ᵇ i
+@[simp] theorem BSubst.id_app : (id x : 𝓛.BTerm n) = #ᵇx := rfl
+@[simp] theorem BTerm.subst_id : t[BSubst.id]ₜᵇ = t := by
+  induction t with simp
+  | func f v ih => ext; apply ih
+
+def BSubst.single (t : 𝓛.BTerm m) : 𝓛.BSubst (m + 1) m :=
+  t ∷ᵥ id
+prefix:max "↦ᵇ " => BSubst.single
+@[simp] theorem BSubst.single_app_zero : (↦ᵇ t) 0 = t := rfl
+@[simp] theorem BSubst.single_app_succ : (↦ᵇ t) x.succ = #ᵇx := rfl
+
+def BSubst.shift : 𝓛.BSubst m (m + 1) := λ x => #ᵇ(Fin.succ x)
+def BTerm.shift (t : 𝓛.BTerm m) := t[BSubst.shift]ₜᵇ
+prefix:max "↑ₜᵇ" => BTerm.shift
+@[simp] theorem BSubst.shift_app : (shift x : 𝓛.BTerm (m + 1)) = #ᵇx.succ := rfl
+@[simp] theorem BTerm.shift_var : ↑ₜᵇ(#ᵇx : 𝓛.BTerm m) = #ᵇx.succ := rfl
+
+def BSubst.assign (t : 𝓛.BTerm (m + 1)) : 𝓛.BSubst (m + 1) (m + 1) :=
+  t ∷ᵥ shift
+prefix:max "≔ᵇ " => BSubst.assign
+@[simp] theorem BSubst.assign_app_zero : (≔ᵇ t) 0 = t := rfl
+@[simp] theorem BSubst.assign_app_succ {x : Fin n} : (≔ᵇ t) x.succ = #ᵇx.succ := rfl
+
+def BSubst.lift (σ : 𝓛.BSubst m k) : 𝓛.BSubst (m + 1) (k + 1) :=
+  #ᵇ0 ∷ᵥ (λ x => ↑ₜᵇ(σ x))
+prefix:max "⇑ᵇ" => BSubst.lift
+@[simp] theorem BSubst.lift_app_zero : ⇑ᵇσ 0 = #ᵇ0 := rfl
+@[simp] theorem BSubst.lift_app_succ : ⇑ᵇσ x.succ = ↑ₜᵇ(σ x) := rfl
+
+theorem BTerm.val_subst_eq {σ : 𝓛.BSubst m k} :
+  (∀ x, (σ x).val = σ' x) → t[σ]ₜᵇ.val = t.val[σ']ₜ := by
+  intro h
+  induction t with simp [subst, h]
+  | func f v ih => ext; apply ih _ h
+
+theorem BTerm.val_shift_eq : (↑ₜᵇt).val = ↑ₜt.val := by
+  apply BTerm.val_subst_eq; intro; rfl
+
+
+
+inductive BFormula (𝓛 : Language) : ℕ → Type where
+| rel : 𝓛.𝓡 n → (Fin n → 𝓛.BTerm m) → 𝓛.BFormula m
+| eq : 𝓛.BTerm m → 𝓛.BTerm m → 𝓛.BFormula m
+| false : 𝓛.BFormula m
+| imp : 𝓛.BFormula m → 𝓛.BFormula m → 𝓛.BFormula m
+| all : 𝓛.BFormula (m + 1) → 𝓛.BFormula m
+
+infix:70 " ⬝ᵣᵇ " => BFormula.rel
+instance : PropNotation (𝓛.BFormula m) := ⟨BFormula.false, BFormula.imp⟩
+prefix:59 "∀ᵇ " => BFormula.all
+abbrev BFormula.exist (p : 𝓛.BFormula (m + 1)) := ~ ∀ᵇ (~ p)
+prefix:59 "∃ᵇ " => BFormula.exist
+
+infix:60 " ≐ᵇ " => BFormula.eq
+
+@[simp] theorem BFormula.false_eq : BFormula.false = (⊥ : 𝓛.BFormula m) := rfl
+@[simp] theorem BFormula.imp_eq : BFormula.imp p q = p ⇒ q := rfl
+
+abbrev Sentence (𝓛 : Language) := 𝓛.BFormula 0
+
+def BFormula.alls : ∀ {m}, 𝓛.BFormula m → 𝓛.Sentence
+| 0, p => p
+| _ + 1, p => (∀ᵇ p).alls
+prefix:59 "∀* " => BFormula.alls
+
+def BFormula.val : 𝓛.BFormula m → 𝓛.Formula
+| p ⬝ᵣᵇ v => p ⬝ᵣ (λ i => (v i).val)
+| t₁ ≐ᵇ t₂ => t₁.val ≐ t₂.val
+| ⊥ => ⊥
+| p ⇒ q => p.val ⇒ q.val
+| ∀ᵇ p => ∀' p.val
+@[simp] theorem BFormula.val_rel : (p ⬝ᵣᵇ v : 𝓛.BFormula m).val = p ⬝ᵣ (λ i => (v i).val) := rfl
+@[simp] theorem BFormula.val_eq : (t₁ ≐ᵇ t₂).val = t₁.val ≐ t₂.val := rfl
+@[simp] theorem BFormula.val_false : (⊥ : 𝓛.BFormula m).val = ⊥ := rfl
+@[simp] theorem BFormula.val_imp : (p ⇒ q : 𝓛.BFormula m).val = p.val ⇒ q.val := rfl
+@[simp] theorem BFormula.val_all : (∀ᵇ p).val = ∀' p.val := rfl
+
+@[simp] def Formula.bound : 𝓛.Formula → ℕ
+| _ ⬝ᵣ v => Vec.max (λ i => (v i).bound)
+| t₁ ≐ t₂ => max t₁.bound t₂.bound
+| ⊥ => 0
+| p ⇒ q => max p.bound q.bound
+| ∀' p => p.bound - 1
+
+theorem BFormula.property : (p : 𝓛.BFormula m).val.bound ≤ m := by
+  induction p with simp
+  | rel r v => apply Vec.max_le; intro; apply BTerm.property
+  | eq t₁ t₂ => simp [BTerm.property]
+  | imp p q ih₁ ih₂ => simp [ih₁, ih₂]
+  | all p ih => simp [ih]
+
+def BFormula.mk :
+  (p : 𝓛.Formula) → m ≥ p.bound → 𝓛.BFormula m
+| r ⬝ᵣ v, h => r ⬝ᵣᵇ (λ i => BTerm.mk (v i) (Nat.le_trans (Vec.le_max (v := Term.bound ∘ v)) h))
+| t₁ ≐ t₂, h => BTerm.mk t₁ (le_of_max_le_left h) ≐ᵇ BTerm.mk t₂ (le_of_max_le_right h)
+| ⊥, _ => ⊥
+| p ⇒ q, h => mk p (le_of_max_le_left h) ⇒ mk q (le_of_max_le_right h)
+| ∀' p, h => ∀ᵇ (mk p (Nat.le_succ_of_pred_le h))
+
+theorem BFormula.val_mk {p : 𝓛.Formula} {h : m ≥ p.bound} :
+  (mk p h).val = p := by
+  induction p generalizing m with simp [mk]
+  | rel => ext; simp [BTerm.val_mk]
+  | eq => simp [BTerm.val_mk]
+  | imp _ _ ih₁ ih₂ => simp [ih₁, ih₂]
+  | all _ ih => simp [ih]
+
+def BFormula.subst : 𝓛.BFormula m → 𝓛.BSubst m k → 𝓛.BFormula k
+| r ⬝ᵣᵇ v, σ => r ⬝ᵣᵇ (λ i => (v i).subst σ)
+| t₁ ≐ᵇ t₂, σ => t₁.subst σ ≐ᵇ t₂.subst σ
+| ⊥, _ => ⊥
+| p ⇒ q, σ => p.subst σ ⇒ q.subst σ
+| ∀ᵇ p, σ => ∀ᵇ (p.subst (⇑ᵇσ))
+notation:80 p "[" σ "]ₚᵇ" => BFormula.subst p σ
+
+@[simp] theorem BFormula.subst_rel : (r ⬝ᵣᵇ v)[σ]ₚᵇ = r ⬝ᵣᵇ (λ i => (v i)[σ]ₜᵇ) := rfl
+@[simp] theorem BFormula.subst_eq : (t₁ ≐ᵇ t₂)[σ]ₚᵇ = t₁[σ]ₜᵇ ≐ᵇ t₂[σ]ₜᵇ := rfl
+@[simp] theorem BFormula.subst_false : ⊥[σ]ₚᵇ = ⊥ := rfl
+@[simp] theorem BFormula.subst_imp : (p ⇒ q)[σ]ₚᵇ = p[σ]ₚᵇ ⇒ q[σ]ₚᵇ := rfl
+@[simp] theorem BFormula.subst_neg : (~ p)[σ]ₚᵇ = ~ p[σ]ₚᵇ := rfl
+@[simp] theorem BFormula.subst_all : (∀ᵇ p)[σ]ₚᵇ = ∀ᵇ p[⇑ᵇσ]ₚᵇ := rfl
+
+def BFormula.shift (p : 𝓛.BFormula m) := p[BSubst.shift]ₚᵇ
+prefix:max "↑ₚᵇ" => BFormula.shift
+
+theorem BFormula.subst_id : p[BSubst.id]ₚᵇ = p := by
+  induction p <;> simp
+  case imp p q ih₁ ih₂ => simp [ih₁, ih₂]
+  case all p ih =>
+    conv => rhs; rw [←ih]
+    congr
+    funext x
+    cases x using Fin.cases
+    · rfl
+    · simp
+
+theorem BFormula.val_subst_eq {σ : 𝓛.BSubst m k} :
+  (∀ x, (σ x).val = σ' x) → p[σ]ₚᵇ.val = p.val[σ']ₚ := by
+  intro h
+  induction p generalizing k σ' <;> try simp
+  case rel r v => ext; simp [BTerm.val_subst_eq h]
+  case eq t₁ t₂ => simp [BTerm.val_subst_eq h]
+  case imp p q ih₁ ih₂ => simp [ih₁ h, ih₂ h]
+  case all p ih =>
+    apply ih
+    intro x
+    cases x using Fin.cases
+    · rfl
+    · simp [BTerm.val_shift_eq, h]
+
+theorem Sentence.val_subst_eq {p : 𝓛.Sentence} :
+  p.val[σ]ₚ = p.val := by
+  rw [←BFormula.val_subst_eq (σ := BSubst.id) (·.elim0), BFormula.subst_id]
+
+theorem Sentence.shift_eq {p : Sentence 𝓛} :
+  ↑ₚp.val = p.val := Sentence.val_subst_eq
+
+end FirstOrder.Language
