MathematicalLogic/FirstOrder/Completeness/Basic.lean
@@ -1,7 +1,0 @@
-import MathematicalLogic.FirstOrder.Proof
-
-def WitnessProperty (Γ : Context 𝓛) :=
-  ∀ p, Γ ⊢ ∃' p → ∃ (c : Const 𝓛), Γ ⊢ p[↦ₛ c]ₚ
-
-def MaximalConsistent (Γ : Context 𝓛) :=
-  Consistent Γ ∧ ∀ p, Γ ⊢ p ∨ Γ ⊢ ~ p
