MathematicalLogic/FirstOrder/Completeness/Completeness.lean
@@ -1,0 +1,55 @@
+import MathematicalLogic.FirstOrder.Theory
+import MathematicalLogic.FirstOrder.Completeness.Henkin
+import MathematicalLogic.FirstOrder.Completeness.Lindenbaum
+import MathematicalLogic.FirstOrder.Completeness.TermModel
+
+namespace FirstOrder.Language
+
+variable {𝓛 : Language} {Γ : 𝓛.Context}
+
+theorem Context.Satisfiable.of_consistent : Γ.Consistent → Γ.Satisfiable := by
+  intro h
+  apply consistency_of_henkin_formulas at h
+  apply lindenbaum at h
+  rcases h with ⟨Δ, h₁, h₂, h₃⟩
+  simp at h₁; rcases h₁ with ⟨h₁, h₁'⟩
+  apply consts_keeps_satisfiability (𝓒 := 𝓛.witOmega)
+  apply Satisfiable.weaken h₁
+  apply satisfiable_by_term_model h₂ h₃
+  exact henkin_formulas_saturated h₁'
+
+theorem completeness : Γ ⊨ p → Γ ⊢ p := by
+  intro h₁
+  apply Proof.mp Proof.double_neg2
+  by_contra h₂
+  rw [←Context.Consistent.append] at h₂
+  apply Context.Satisfiable.of_consistent at h₂
+  rcases h₂ with ⟨𝓜, ρ, h₂⟩
+  have h₃ := h₂ (~ p) (Set.mem_insert _ _)
+  simp [Formula.interp_neg] at h₃
+  apply h₃
+  apply h₁
+  intros q h
+  apply h₂
+  exact Set.mem_insert_of_mem _ h
+
+theorem compactness : Γ ⊨ p → ∃ Δ, Δ ⊆ Γ ∧ Δ.Finite ∧ Δ ⊨ p := by
+  intro h
+  apply completeness at h
+  apply Proof.compactness at h
+  rcases h with ⟨Δ, h₁, h₂, h₃⟩
+  apply soundness at h₃
+  exists Δ
+
+theorem Theory.Satisfiable.of_consistent {𝓣 : 𝓛.Theory} :
+  𝓣.Consistent → 𝓣.Satisfiable := by
+  intro h
+  apply Context.Satisfiable.of_consistent at h
+  rcases h with ⟨𝓢, ρ, h⟩
+  exists 𝓢
+  intros p h'
+  rw [Sentence.val_interp_eq]
+  apply h
+  exists p
+
+end FirstOrder.Language
