MathematicalLogic/FirstOrder/Completeness/Defs.lean
@@ -1,0 +1,11 @@
+import MathematicalLogic.FirstOrder.Proof
+
+namespace FirstOrder.Language.Context
+
+variable {𝓛 : Language} (Γ : 𝓛.Context)
+
+def Saturated := ∀ p, Γ ⊢ ∃' p → ∃ (c : 𝓛.Const), Γ ⊢ p[↦ₛ c]ₚ
+
+def Complete := ∀ p, Γ ⊢ p ∨ Γ ⊢ ~ p
+
+end FirstOrder.Language.Context
