MathematicalLogic/FirstOrder/Completeness/Henkin.lean
@@ -1,0 +1,838 @@
+import Mathlib.Data.List.Sort
+import MathematicalLogic.FirstOrder.Semantics
+import MathematicalLogic.FirstOrder.Completeness.Defs
+
+lemma Set.Finite.induction_on_sorted
+  {C : Set α → Prop} {S : Set α} (h : S.Finite)
+  (r : α → α → Prop) [DecidableRel r] [IsTrans α r] [IsTotal α r]
+  (H0 : C ∅)
+  (H1 : ∀ {a s}, a ∈ S → s ⊆ S → a ∉ s → (∀ x ∈ s, r a x) → C s → C (insert a s)) :
+  C S := by
+  lift S to Finset α using h
+  rcases S with ⟨S, h₁⟩
+  unfold Finset.toSet at *; simp at *
+  generalize h : List.insertionSort r S.toList = l
+  replace h₁ : l.Nodup := by
+    rw [←h, List.Perm.nodup_iff (List.perm_insertionSort _ _)]
+    simp [←Multiset.coe_nodup]
+    exact h₁
+  have h₂ : l.Sorted r := by
+    rw [←h]
+    apply List.sorted_insertionSort
+  have h₃ : ∀ x, x ∈ l ↔ x ∈ S := by
+    intro x
+    rw [←h, ←Multiset.mem_toList]
+    apply List.Perm.mem_iff
+    apply List.perm_insertionSort
+  simp [←h₃]
+  replace h₃ : ∀ x, x ∈ l → x ∈ S := by
+    simp [h₃]
+  clear h
+  induction' h₂ with a l h₂ _ ih
+  · simp; apply H0
+  · simp; change C (insert a { x | x ∈ l })
+    apply H1
+    · apply h₃; simp
+    · intros x h; apply h₃; right; exact h
+    · intro h
+      cases' h₁ with _ _ h₁
+      exact h₁ _ h rfl
+    · exact h₂
+    · apply ih
+      · cases' h₁ with _ _ _ h₁
+        exact h₁
+      · intros x h; apply h₃; right; exact h
+
+lemma Set.decompose_subset_union {s₁ s₂ s₃ : Set α} :
+  s₁ ⊆ s₂ ∪ s₃ → ∃ s₄ s₅, s₁ = s₄ ∪ s₅ ∧ s₄ ⊆ s₂ ∧ s₅ ⊆ s₃ := by
+  intros h
+  exists s₁ ∩ s₂
+  exists s₁ ∩ s₃
+  aesop
+
+
+
+namespace FirstOrder.Language
+
+@[reducible]
+def addConsts (𝓛 : Language) (𝓒 : Type) [DecidableEq 𝓒] : Language where
+  𝓕 := λ
+       | 0 => 𝓛.𝓕 0 ⊕ 𝓒
+       | n + 1 => 𝓛.𝓕 (n + 1)
+  decEq𝓕 :=
+    @λ
+    | 0, f, g => Sum.instDecidableEqSum f g
+    | _ + 1, _, _ => inferInstance
+  𝓡 := 𝓛.𝓡
+local infix:70 " ⊎ " => Language.addConsts
+
+variable {𝓛 : Language} {𝓒 : Type} [DecidableEq 𝓒]
+
+def Term.injConsts : 𝓛.Term → (𝓛 ⊎ 𝓒).Term
+| #x => #x
+| Term.func (n := 0) f ([]ᵥ) => Sum.inl f ⬝ₜ []ᵥ
+| Term.func (n := _ + 1) f v => f ⬝ₜ λ i => (v i).injConsts
+
+local notation "⌈" t "⌉ₜ" => Term.injConsts t
+
+def Formula.injConsts : 𝓛.Formula → (𝓛 ⊎ 𝓒).Formula
+| r ⬝ᵣ v => r ⬝ᵣ λ i => (v i).injConsts
+| t₁ ≐ t₂ => t₁.injConsts ≐ t₂.injConsts
+| ⊥ => ⊥
+| p ⇒ q => p.injConsts ⇒ q.injConsts
+| ∀' p => ∀' p.injConsts
+
+local notation "⌈" p "⌉ₚ" => Formula.injConsts p
+
+def Context.injConsts (Γ : 𝓛.Context) : (𝓛 ⊎ 𝓒).Context :=
+  { ⌈p⌉ₚ | p ∈ Γ }
+
+local notation "⌈" Γ "⌉ᴳ" => Context.injConsts Γ
+
+def Term.eraseConsts : (𝓛 ⊎ 𝓒).Term → ℕ → 𝓛.Term
+| #x, _ => #x
+| func (n := 0) (Sum.inl f) []ᵥ, _ => f ⬝ₜ []ᵥ
+| func (n := 0) (Sum.inr _) []ᵥ, x => #x
+| func (n := _ + 1) f v, x => f ⬝ₜ λ i => (v i).eraseConsts x
+local notation "⌊" t "⌋ₜ" => Term.eraseConsts t
+
+def Formula.eraseConsts : (𝓛 ⊎ 𝓒).Formula → ℕ → 𝓛.Formula
+| r ⬝ᵣ v, x => r ⬝ᵣ λ i => ⌊v i⌋ₜ x
+| t₁ ≐ t₂, x => ⌊t₁⌋ₜ x ≐ ⌊t₂⌋ₜ x
+| ⊥, _ => ⊥
+| p ⇒ q, x => p.eraseConsts x ⇒ q.eraseConsts x
+| ∀' p, x => ∀' (p.eraseConsts (x + 1))
+local notation "⌊" p "⌋ₚ" => Formula.eraseConsts p
+
+lemma Term.erase_inj : ⌊(⌈t⌉ₜ : (𝓛 ⊎ 𝓒).Term)⌋ₜ x = t := by
+  induction t with
+  | var x => simp [injConsts, eraseConsts]
+  | @func n f v ih =>
+    cases n with simp [injConsts, eraseConsts]
+    | zero => simp [Vec.eq_nil]
+    | succ => ext; simp [ih]
+
+lemma Formula.erase_inj : ⌊(⌈p⌉ₚ : (𝓛 ⊎ 𝓒).Formula)⌋ₚ x = p := by
+  induction p generalizing x with simp [injConsts, eraseConsts]
+  | rel r v => simp [Term.erase_inj]
+  | eq t₁ t₂ => simp [Term.erase_inj]
+  | imp _ _ ih₁ ih₂ => simp [ih₁, ih₂]
+  | all _ ih => simp [ih]
+  
+section
+
+variable {t : (𝓛 ⊎ 𝓒).Term} {σ₁ : (𝓛 ⊎ 𝓒).Subst} {σ₂ : 𝓛.Subst}
+  (h₁ : ∀ z, σ₂ z = ⌊σ₁ z⌋ₜ x) (h₂ : σ₂ y = #x)
+
+lemma Term.erase_swap_subst : ⌊t[σ₁]ₜ⌋ₜ x = (⌊t⌋ₜ y)[σ₂]ₜ := by
+  induction t with
+  | var z => simp [eraseConsts, h₁]
+  | @func n f v ih =>
+    cases n with
+    | zero => cases f <;> simp [eraseConsts, h₂, Vec.eq_nil]
+    | succ => simp [eraseConsts]; ext; simp [ih]
+
+lemma Formula.erase_swap_subst : ⌊p[σ₁]ₚ⌋ₚ x = (⌊p⌋ₚ y)[σ₂]ₚ := by
+  induction p generalizing σ₁ σ₂ x y with simp [eraseConsts]
+  | rel r v | eq t₁ t₂ => simp [Term.erase_swap_subst h₁ h₂]
+  | imp p q ih₁ ih₂ => simp [ih₁ h₁ h₂, ih₂ h₁ h₂]
+  | all p ih =>
+    rw [ih]
+    · intro z; cases z
+      · rfl
+      · simp [Term.shift]
+        rw [h₁, Term.erase_swap_subst]
+        · simp [Term.eraseConsts]
+        · rfl
+    · simp [h₂, Term.shift]
+
+end
+
+lemma erase_keeps_axioms {p : (𝓛 ⊎ 𝓒).Formula} :
+  p ∈ (𝓛 ⊎ 𝓒).Axioms → ⌊p⌋ₚ x ∈ 𝓛.Axioms := by
+  intro h
+  induction h generalizing x <;> simp [Formula.eraseConsts] <;> try constructor
+  case a4 t p =>
+    rw [Formula.erase_swap_subst (σ₂ := ↦ₛ (⌊t⌋ₜ x))]
+    · exact .a4
+    · intro z; cases z <;> simp [Term.eraseConsts]
+    · rfl
+  case a5 p =>
+    rw [Formula.shift, Formula.erase_swap_subst]
+    · exact .a5
+    · intro z; simp [Term.eraseConsts]
+    · rfl
+  case e2 t₁ t₂ p =>
+    rw [Formula.erase_swap_subst (y := x + 1), Formula.erase_swap_subst (y := x + 1)]
+    · exact .e2
+    · intro z; cases z <;> simp [Term.eraseConsts]
+    · rfl
+    · intro z; cases z <;> simp [Term.eraseConsts]
+    · rfl
+  case all ih =>
+    apply ih
+
+lemma erase_keeps_proof {p : (𝓛 ⊎ 𝓒).Formula} : ⌈Γ⌉ᴳ ⊢ p → Γ ⊢ ⌊p⌋ₚ x := by
+  intro h
+  induction h with
+  | hyp h =>
+    rcases h with ⟨p', ⟨h₁, h₂⟩⟩
+    subst h₂
+    simp [Formula.erase_inj]
+    exact Proof.hyp h₁
+  | ax h =>
+    apply Proof.ax
+    apply erase_keeps_axioms
+    exact h
+  | mp _ _ ih₁ ih₂ =>
+    exact ih₁.mp ih₂
+
+theorem consts_keeps_consistency {Γ : 𝓛.Context} :
+  Γ.Consistent → (⌈Γ⌉ᴳ : (𝓛 ⊎ 𝓒).Context).Consistent := by
+  intros h h₁
+  apply erase_keeps_proof (x := 0) at h₁
+  apply h
+  exact h₁
+
+def Structure.reductConsts (𝓜 : (𝓛 ⊎ 𝓒).Structure) : 𝓛.Structure where
+  𝓤 := 𝓜.𝓤
+  inhabited𝓤 := inferInstance
+  interp𝓕 :=
+    @λ
+    | 0, f => 𝓜.interp𝓕 (Sum.inl f)
+    | _ + 1, f => 𝓜.interp𝓕 f
+  interp𝓡 := 𝓜.interp𝓡
+local notation "⌊" 𝓜 "⌋ₘ" => Structure.reductConsts 𝓜
+
+lemma Term.interp_reduct : ⟦ t ⟧ₜ ⌊𝓜⌋ₘ, ρ = ⟦ (⌈t⌉ₜ : (𝓛 ⊎ 𝓒).Term) ⟧ₜ 𝓜, ρ := by
+  induction t with
+  | var x => rfl
+  | @func n f v ih =>
+    cases n with simp [injConsts, interp]
+    | zero => simp [Vec.eq_nil]; rfl
+    | succ => simp [ih]; rfl
+
+lemma Formula.interp_reduct :
+  ⌊𝓜⌋ₘ ⊨[ρ] p ↔ 𝓜 ⊨[ρ] (⌈p⌉ₚ : (𝓛 ⊎ 𝓒).Formula) := by
+  induction p generalizing ρ with simp [injConsts, interp]
+  | rel r v => simp [Term.interp_reduct]; rfl
+  | eq t₁ t₂ => simp [Term.interp_reduct]
+  | imp p q ih₁ ih₂ => simp [ih₁, ih₂]
+  | all p ih => apply forall_congr'; intro; rw [ih]; rfl
+
+theorem consts_keeps_satisfiability :
+  Context.Satisfiable.{u} (⌈Γ⌉ᴳ : (𝓛 ⊎ 𝓒).Context) → Context.Satisfiable.{u} Γ := by
+  rintro ⟨𝓜, ⟨ρ, h⟩⟩
+  exists ⌊𝓜⌋ₘ
+  exists ρ
+  intros p h₁
+  rw [Formula.interp_reduct]
+  apply h
+  exists p
+
+
+
+def Term.consts : 𝓛.Term → Set 𝓛.Const
+| #_ => {}
+| Term.func (n := 0) c ([]ᵥ) => {c}
+| Term.func (n := _ + 1) _ v => ⋃i, (v i).consts
+
+def Formula.consts : 𝓛.Formula → Set 𝓛.Const
+| _ ⬝ᵣ v => ⋃i, (v i).consts
+| t₁ ≐ t₂ => t₁.consts ∪ t₂.consts
+| ⊥ => {}
+| p ⇒ q => p.consts ∪ q.consts
+| ∀' p => p.consts
+
+lemma Term.consts_of_subst :
+  t[σ]ₜ.consts = t.consts ∪ ⋃ x ∈ t.vars, (σ x).consts := by
+  induction t with
+  | var x => simp [vars, consts]
+  | @func n f v ih =>
+    cases n with simp [vars, Term.consts]
+    | succ => rw [Set.iUnion_comm, ←Set.iUnion_union_distrib]; simp_rw [ih]
+
+lemma Formula.consts_of_subst :
+  p[σ]ₚ.consts = p.consts ∪ ⋃ x ∈ p.free, (σ x).consts := by
+  induction p generalizing σ with simp_rw [free, consts]
+  | rel r v => simp_rw [Set.biUnion_iUnion, ←Set.iUnion_union_distrib, Term.consts_of_subst]
+  | eq t₁ t₂ => simp_rw [Set.biUnion_union, Term.consts_of_subst]; aesop
+  | false => simp
+  | imp p q ih₁ ih₂ => rw [ih₁, ih₂, Set.biUnion_union]; aesop
+  | all p ih =>
+    ext c; simp [ih]; apply or_congr_right
+    constructor
+    · rintro ⟨x, h₁, h₂⟩
+      cases x with
+      | zero => contradiction
+      | succ x =>
+        simp [Term.shift, Term.consts_of_subst] at h₂
+        rcases h₂ with (h₂ | ⟨_, _, h₃⟩)
+        · exists x
+        · simp [Term.consts] at h₃
+    · rintro ⟨y, ⟨h₁, h₂⟩⟩
+      exists y + 1
+      constructor
+      · exact h₁
+      · simp [Term.shift, Term.consts_of_subst]
+        left; exact h₂
+
+def Term.substConst : 𝓛.Term → 𝓛.Const → ℕ → 𝓛.Term
+| #x, _, y =>
+  if x < y then #x else #(x + 1)
+| Term.func (n := 0) c ([]ᵥ), c', x =>
+  if c = c' then #x else c
+| Term.func (n := _ + 1) f v, c, x => f ⬝ₜ λ i => (v i).substConst c x
+local notation t "[" c " ↦ᶜ " x "]ₜ" => Term.substConst t c x
+
+def Formula.substConst : 𝓛.Formula → 𝓛.Const → ℕ → 𝓛.Formula
+| r ⬝ᵣ v, c, x => r ⬝ᵣ λ i => (v i)[c ↦ᶜ x]ₜ
+| t₁ ≐ t₂, c, x => t₁[c ↦ᶜ x]ₜ ≐ t₂[c ↦ᶜ x]ₜ
+| ⊥, _, _ => ⊥
+| p ⇒ q, c, x => p.substConst c x ⇒ q.substConst c x
+| ∀' p, c, x => ∀' (p.substConst c (x + 1))
+local notation p "[" c " ↦ᶜ " x "]ₚ" => Formula.substConst p c x
+
+def Subst.shift_since (x : ℕ) : 𝓛.Subst := λ y => if y < x then #y else #(y + 1)
+
+lemma Term.subst_const_of_non_const_aux :
+  c ∉ t.consts → t[c ↦ᶜ x]ₜ = t[Subst.shift_since x]ₜ := by
+  intro h
+  induction t with
+  | var y => simp [substConst, Subst.shift_since]
+  | @func n f v ih =>
+    cases n with (simp [consts] at h; simp [substConst])
+    | zero => simp [Ne.symm h, Vec.eq_nil]
+    | succ n => ext; apply ih; apply h
+
+lemma Formula.subst_const_of_non_const_aux :
+  c ∉ p.consts → p[c ↦ᶜ x]ₚ = p[Subst.shift_since x]ₚ := by
+  intro h
+  induction p generalizing x with (simp [consts, not_or] at h; simp [substConst])
+  | rel r v => ext; apply Term.subst_const_of_non_const_aux; apply h
+  | eq t₁ t₂ => constructor <;> apply Term.subst_const_of_non_const_aux <;> aesop
+  | imp p q ih₁ ih₂ => rw [ih₁ h.left, ih₂ h.right]
+  | all p ih =>
+    rw [ih h]
+    congr
+    funext y
+    cases y with simp [Subst.shift_since]
+    | succ y =>
+      by_cases h : y < x
+      · simp [h, Nat.succ_lt_succ h, Term.shift]
+      · simp [h, mt Nat.lt_of_succ_lt_succ h, Term.shift]
+
+lemma Formula.subst_const_of_non_const : c ∉ p.consts → p[c ↦ᶜ 0]ₚ = ↑ₚp :=
+  subst_const_of_non_const_aux
+
+section
+
+variable {c : 𝓛.Const} {σ₁ σ₂ : 𝓛.Subst}
+  (h₁ : ∀ z, σ₂ (if z < y then z else z + 1) = (σ₁ z)[c ↦ᶜ x]ₜ) (h₂ : σ₂ y = #x)
+
+lemma Term.subst_const_swap_subst : t[σ₁]ₜ[c ↦ᶜ x]ₜ = t[c ↦ᶜ y]ₜ[σ₂]ₜ := by
+  induction t with
+  | var z => simp [substConst, ←h₁]; by_cases h : z < y <;> simp [h]
+  | @func n f v ih =>
+    cases n with simp [substConst]
+    | zero => by_cases h : f = c <;> simp [h, h₂, Vec.eq_nil]
+    | succ n => ext; apply ih
+
+lemma Formula.subst_const_swap_subst : p[σ₁]ₚ[c ↦ᶜ x]ₚ = p[c ↦ᶜ y]ₚ[σ₂]ₚ := by
+  induction p generalizing σ₁ σ₂ x y with simp [substConst]
+  | rel r v => ext; simp [Term.subst_const_swap_subst h₁ h₂]
+  | eq t₁ t₂ => simp [Term.subst_const_swap_subst h₁ h₂]
+  | imp p q ih₁ ih₂ => rw [ih₁ h₁ h₂, ih₂ h₁ h₂]
+  | all p ih =>
+    rw [ih]
+    · intro z
+      cases z with
+      | zero => simp [Term.substConst]
+      | succ z =>
+        replace h₁ := h₁ z
+        by_cases h : z < y
+        · simp [h] at h₁
+          simp [Nat.succ_lt_succ h, h₁, Term.shift]
+          rw [Term.subst_const_swap_subst]
+          · intro z'; simp [Term.substConst]
+            by_cases h : z' < x <;> simp [h]
+          · rfl
+        · simp [h] at h₁
+          simp [mt Nat.lt_of_succ_lt_succ h,  h₁, Term.shift]
+          rw [Term.subst_const_swap_subst]
+          · intro z'; simp [Term.substConst]
+            by_cases h : z' < x <;> simp [h]
+          · rfl
+    · simp [h₂, Term.shift]
+
+end
+
+theorem subst_const_keeps_axioms :
+  p ∈ 𝓛.Axioms → p[c ↦ᶜ x]ₚ ∈ 𝓛.Axioms := by
+  intro h
+  induction h generalizing x <;> simp [Formula.substConst] <;> try constructor
+  case a4 t p =>
+    rw [Formula.subst_const_swap_subst (σ₂ := ↦ₛ (t[c ↦ᶜ x]ₜ))]
+    · exact .a4
+    · intro z
+      cases z with simp
+      | succ z =>
+        by_cases h : z < x
+        · simp [h, Nat.succ_lt_succ h, Term.substConst]
+        · simp [h, mt Nat.lt_of_succ_lt_succ h, Term.substConst]
+    · rfl
+  case a5 p =>
+    rw [Formula.shift, Formula.subst_const_swap_subst (σ₂ := Subst.shift)]
+    · exact .a5
+    · intro z
+      by_cases h : z < x <;> simp [h, Term.substConst]
+    · rfl
+  case e2 t₁ t₂ =>
+    rw [Formula.subst_const_swap_subst (y := x + 1), Formula.subst_const_swap_subst (y := x + 1)]
+    · exact .e2
+    · intro z
+      cases z with simp
+      | succ z =>
+        by_cases h : z < x
+        · simp [h, Nat.succ_lt_succ h, Term.substConst]
+        · simp [h, mt Nat.lt_of_succ_lt_succ h, Term.substConst]
+    · simp
+    · intro z
+      cases z with simp
+      | succ z =>
+        by_cases h : z < x
+        · simp [h, Nat.succ_lt_succ h, Term.substConst]
+        · simp [h, mt Nat.lt_of_succ_lt_succ h, Term.substConst]
+    · simp
+  case all ih =>
+    apply ih
+
+theorem subst_const_keeps_proof {p : 𝓛.Formula} :
+  (∀ p ∈ Γ, c ∉ p.consts) → Γ ⊢ p → Γ ⊢ ∀' p[c ↦ᶜ 0]ₚ := by
+  intros h₁ h
+  induction h with
+  | hyp h =>
+    rw [Formula.subst_const_of_non_const (h₁ _ h)]
+    apply Proof.mp (Proof.ax .a5)
+    exact Proof.hyp h
+  | ax h =>
+    apply Proof.ax
+    apply Axioms.all
+    apply subst_const_keeps_axioms
+    exact h
+  | mp _ _ ih₁ ih₂ =>
+    exact Proof.mp2 (Proof.ax .a6) ih₁ ih₂
+
+theorem const_generalization {c : 𝓛.Const} :
+  (∀ p ∈ Γ, c ∉ p.consts) → c ∉ p.consts → Γ ⊢ p[↦ₛ c]ₚ → Γ ⊢ ∀' p := by
+  intros h₁ h₂ h₃
+  apply subst_const_keeps_proof h₁ at h₃
+  rw [Formula.subst_const_swap_subst (σ₂ := (↦ₛ #0))] at h₃
+  · rw [Formula.subst_const_of_non_const h₂, Formula.shift_subst_single] at h₃; exact h₃
+  · intro z; cases z <;> simp [Term.substConst]
+  · rfl
+
+
+
+def witAccAux (𝓛 : Language) : (n : ℕ) → Σ (T : Type), DecidableEq T
+| 0 => ⟨Empty, inferInstance⟩
+| n + 1 =>
+  let ⟨𝓛', _⟩ := 𝓛.witAccAux n
+  ⟨𝓛' ⊕ (𝓛 ⊎ 𝓛').Formula, inferInstance⟩
+
+def witAcc (𝓛 : Language) (n : ℕ) := (𝓛.witAccAux n).fst
+instance : DecidableEq (𝓛.witAcc n) := (𝓛.witAccAux n).snd
+@[reducible] def witNth (𝓛 : Language) (n : ℕ) : Type := (𝓛 ⊎ 𝓛.witAcc n).Formula
+
+@[reducible] def addWitNth (𝓛 n) := 𝓛 ⊎ 𝓛.witAcc n
+local instance : Pow Language ℕ where
+  pow := addWitNth
+
+@[reducible] def witOmega (𝓛 : Language) : Type := Σ n, 𝓛.witNth n
+@[reducible] def addWitOmega (𝓛 : Language) := 𝓛 ⊎ 𝓛.witOmega
+local postfix:max "*" => Language.addWitOmega
+
+def injWitOmega : {n : ℕ} → 𝓛.witAcc n → 𝓛.witOmega
+| _ + 1, Sum.inl c => injWitOmega c
+| n + 1, Sum.inr c => ⟨n, c⟩
+
+def Term.injOmega {n : ℕ} : (𝓛^n).Term → (𝓛*).Term
+| #x => #x
+| Term.func (n := 0) (Sum.inl f) ([]ᵥ) => Sum.inl f ⬝ₜ []ᵥ
+| Term.func (n := 0) (Sum.inr c) ([]ᵥ) => Sum.inr (injWitOmega c) ⬝ₜ []ᵥ
+| Term.func (n := _ + 1) f v => f ⬝ₜ λ i => (v i).injOmega
+
+def Formula.injOmega {n : ℕ} : (𝓛^n).Formula → (𝓛*).Formula
+| r ⬝ᵣ v => r ⬝ᵣ λ i => (v i).injOmega
+| t₁ ≐ t₂ => t₁.injOmega ≐ t₂.injOmega
+| ⊥ => ⊥
+| p ⇒ q => p.injOmega ⇒ q.injOmega
+| ∀' p => ∀' (p.injOmega)
+
+def Term.level : (𝓛*).Term → ℕ
+| #_ => 0
+| Term.func (n := 0) (Sum.inl _) ([]ᵥ) => 0
+| Term.func (n := 0) (Sum.inr c) ([]ᵥ) => c.fst + 1
+| Term.func (n := _ + 1) _ v => Vec.max λ i => (v i).level
+
+def Formula.level : (𝓛*).Formula → ℕ
+| _ ⬝ᵣ v => Vec.max λ i => (v i).level
+| t₁ ≐ t₂ => max t₁.level t₂.level
+| ⊥ => 0
+| p ⇒ q => max p.level q.level
+| ∀' p => p.level
+
+lemma Term.const_less_than_level {t : (𝓛*).Term} :
+  Sum.inr ⟨k, q⟩ ∈ t.consts → k < t.level := by
+  intro h
+  induction t with
+  | var x => simp [consts] at h
+  | @func n f v ih =>
+    cases n with simp [consts] at h
+    | zero => subst h; simp [level]
+    | succ n =>
+      simp [level]
+      rcases h with ⟨i, h⟩
+      apply le_trans' Vec.le_max
+      apply ih; exact h
+
+lemma Formula.const_less_than_level {p : (𝓛*).Formula} :
+  Sum.inr ⟨k, q⟩ ∈ p.consts → k < p.level := by
+  intro h
+  induction p with (simp [consts] at h <;> simp [level])
+  | rel r v =>
+    rcases h with ⟨i, h⟩
+    apply le_trans' Vec.le_max
+    apply Term.const_less_than_level
+    exact h
+  | eq t₁ t₂ =>
+    cases h with
+    | inl h => left; apply Term.const_less_than_level; exact h
+    | inr h => right; apply Term.const_less_than_level; exact h
+  | imp p q ih₁ ih₂ =>
+    cases h with
+    | inl h => left; apply ih₁; exact h
+    | inr h => right; apply ih₂; exact h
+  | all p ih => apply ih; exact h
+
+lemma Term.level_of_inj_consts {t : 𝓛.Term} : ⌈t⌉ₜ.level = 0 := by
+  induction t with
+  | var => simp [injConsts, level]
+  | @func n f v ih =>
+    cases n with simp [injConsts, level]
+    | succ n => simp [ih]
+
+lemma Formula.level_of_inj_consts {p : 𝓛.Formula} : ⌈p⌉ₚ.level = 0 := by
+  induction p with simp [injConsts, level]
+  | rel r v | eq t₁ t₂ => simp [Term.level_of_inj_consts]
+  | imp p q ih₁ ih₂ => simp [ih₁, ih₂]
+  | all p ih => exact ih
+
+lemma level_of_inj_wit_omega {c : 𝓛.witAcc n} : (injWitOmega c).fst < n := by
+  induction n with
+  | zero => cases c
+  | succ n ih =>
+    cases c with simp [injWitOmega]
+    | inl c => exact Nat.lt_of_lt_of_le ih (Nat.le_succ _)
+
+lemma Term.level_of_inj_omega {n : ℕ} {t : (𝓛^n).Term} : t.injOmega.level ≤ n := by
+  induction t with
+  | var => simp [injOmega, level]
+  | @func n f v ih =>
+    cases n with
+    | zero => cases f <;> simp [injOmega, level]; exact level_of_inj_wit_omega
+    | succ n => simp [injOmega, level]; apply Vec.max_le; exact ih
+
+theorem Formula.level_of_inj_omega {n : ℕ} {p : (𝓛^n).Formula} : p.injOmega.level ≤ n := by
+  induction p with simp [injOmega, level]
+  | rel r v => apply Vec.max_le; intro; exact Term.level_of_inj_omega
+  | eq t₁ t₂ => constructor <;> exact Term.level_of_inj_omega
+  | imp p q ih₁ ih₂ => exact ⟨ih₁, ih₂⟩
+  | all p ih => exact ih
+
+lemma Term.le_level_of_subst :
+  n ≤ (t[σ]ₜ).level → n ≤ t.level ∨ ∃ x ∈ t.vars, n ≤ (σ x).level := by
+  intro h
+  induction t with
+  | var x => simp [vars, level]; right; exact h
+  | @func n f v ih =>
+    cases n with
+    | zero => cases f <;> simp [subst, vars, level] at * <;> exact h
+    | succ n =>
+      simp [subst, vars, level, Vec.le_max_iff] at *
+      rcases h with ⟨i, h⟩
+      apply ih at h
+      aesop
+
+lemma Formula.le_level_of_subst :
+  n ≤ (p[σ]ₚ).level → n ≤ p.level ∨ ∃ x ∈ p.free, n ≤ (σ x).level := by
+  intro h
+  induction p generalizing σ with simp [Formula.free, Formula.level] at *
+  | @rel n r v =>
+    cases n with
+    | zero => simp [Vec.max] at *; exact h
+    | succ n =>
+      simp [Vec.le_max_iff] at *
+      rcases h with ⟨i, h⟩
+      apply Term.le_level_of_subst at h
+      aesop
+  | eq t₁ t₂ => rcases h with (h | h) <;> apply Term.le_level_of_subst at h <;> aesop
+  | false => exact h
+  | imp p q ih₁ ih₂ =>
+    rcases h with (h | h)
+    · apply ih₁ at h; aesop
+    · apply ih₂ at h; aesop
+  | all p ih =>
+    rcases ih h with h | ⟨x, h, h'⟩
+    · left; exact h
+    · cases x with
+      | zero => simp [Term.level] at h'; simp [h']
+      | succ x =>
+        simp [Term.shift] at h'
+        apply Term.le_level_of_subst at h'
+        rcases h' with h' | ⟨y, _, h'⟩
+        · right; exists x
+        · simp [Term.level] at h'; simp [h']
+
+lemma Term.level_of_subst_le :
+  (t[σ]ₜ).level ≤ n → t.level ≤ n ∧ ∀ x ∈ t.vars, (σ x).level ≤ n := by
+  intro h
+  induction t with
+  | var x => simp [subst, vars, level] at *; exact h
+  | @func n f v ih =>
+    cases n with
+    | zero => cases f <;> simp [vars, Vec.eq_nil] at * <;> exact h
+    | succ n =>
+      simp [vars, level, Vec.max_le_iff] at *
+      constructor
+      · intro i; exact (ih _ (h _)).left
+      · intros x i h'; exact (ih _ (h _)).right _ h'
+
+lemma Formula.level_of_subst_le :
+  (p[σ]ₚ).level ≤ n → p.level ≤ n ∧ ∀ x ∈ p.free, (σ x).level ≤ n := by
+  intro h
+  induction p generalizing σ with simp [free, level] at *
+  | rel r v =>
+    simp [Vec.max_le_iff] at *
+    constructor
+    · intro i; exact (Term.level_of_subst_le (h _)).left
+    · intros x i h'; exact (Term.level_of_subst_le (h _)).right _ h'
+  | eq t₁ t₂ =>
+    rcases h with ⟨h₁, h₂⟩
+    apply Term.level_of_subst_le at h₁
+    apply Term.level_of_subst_le at h₂
+    aesop
+  | imp p q ih₁ ih₂ =>
+    rcases h with ⟨h₁, h₂⟩
+    apply ih₁ at h₁
+    apply ih₂ at h₂
+    aesop
+  | all p ih =>
+    rcases ih h with ⟨h₁, h₂⟩
+    constructor
+    · exact h₁
+    · intros x h
+      replace h₂ := h₂ _ h
+      simp [Term.shift] at h₂
+      exact (Term.level_of_subst_le h₂).left
+
+lemma exists_inj_wit_omega {c : 𝓛.witOmega} :
+  c.fst + 1 ≤ n → ∃ (c' : 𝓛.witAcc n), c = injWitOmega c' := by
+  cases' c with k c
+  simp
+  intro h
+  induction' h with n _ ih
+  · exists Sum.inr c
+  · rcases ih with ⟨c', h⟩
+    exists Sum.inl c'
+
+lemma Term.exists_inj_omega :
+  t.level ≤ n → ∃ (t' : Term (𝓛^n)), t = t'.injOmega := by
+  intro h
+  induction t with
+  | var x => exists #x
+  | @func n f v ih =>
+    cases n with
+    | zero =>
+      simp [Vec.eq_nil] at *
+      cases f with
+      | inl f => exists Sum.inl f ⬝ₜ []ᵥ
+      | inr c =>
+        simp [level] at h
+        rcases exists_inj_wit_omega h with ⟨c', h⟩
+        exists Sum.inr c' ⬝ₜ []ᵥ
+        simp [h, injOmega]
+    | succ n =>
+      simp [level, Vec.max_le_iff] at h
+      choose v h using λ i => ih _ (h i)
+      exists f ⬝ₜ v
+      simp [injOmega]; ext; simp [h]
+
+lemma Formula.exists_inj_omega :
+  p.level ≤ n → ∃ (p' : Formula (𝓛^n)), p = p'.injOmega := by
+  intro h
+  induction p with simp [level] at h
+  | rel r v =>
+    simp [Vec.max_le_iff] at h
+    choose v h using λ i => Term.exists_inj_omega (h i)
+    exists r ⬝ᵣ v
+    simp [injOmega]; ext; simp [h]
+  | eq t₁ t₂ =>
+    rcases h with ⟨h₁, h₂⟩
+    rcases Term.exists_inj_omega h₁ with ⟨t₁', h₁⟩
+    rcases Term.exists_inj_omega h₂ with ⟨t₂', h₂⟩
+    exists t₁' ≐ t₂'
+    simp [injOmega, h₁, h₂]
+  | false => exists ⊥
+  | imp p q ih₁ ih₂ =>
+    rcases h with ⟨h₁, h₂⟩
+    rcases ih₁ h₁ with ⟨p', h₁⟩
+    rcases ih₂ h₂ with ⟨q', h₂⟩
+    exists p' ⇒ q'
+    simp [injOmega, h₁, h₂]
+  | all p ih =>
+    rcases ih h with ⟨p', h⟩
+    exists ∀' p'
+    simp [injOmega, h]
+
+
+
+def HenkinFormulas (𝓛 : Language) : (𝓛*).Context
+  := { p | ∃ (p' : (𝓛*).Formula) (c : (𝓛*).Const) (n : ℕ) (p'' : (𝓛^n).Formula),
+             p = ∃' p' ⇒ p' [↦ₛ c]ₚ ∧ p' = p''.injOmega ∧ c = Sum.inr ⟨n, p''⟩ ∧ 0 ∈ p'.free }
+
+section
+
+variable {p p' : (𝓛*).Formula} {p'' : (𝓛^n).Formula} {c : (𝓛*).Const}
+  (h₁ : p = ∃' p' ⇒ p' [↦ₛ c]ₚ) (h₂ : p' = p''.injOmega)
+  (h₃ : c = Sum.inr ⟨n, p''⟩) (h₄ : 0 ∈ p'.free)
+
+lemma level_of_henkin_formula : p.level = n + 1 := by
+  subst h₁
+  apply Nat.le_antisymm
+  · simp [Formula.level]
+    have h : Formula.level p' ≤ n := by
+      rw [h₂]; apply Formula.level_of_inj_omega
+    constructor
+    · exact Nat.le_succ_of_le h
+    · apply Nat.le_of_not_lt
+      intro h'
+      apply Formula.le_level_of_subst at h'
+      rcases h' with h' | ⟨x, h', h''⟩
+      · apply Nat.not_le_of_lt h'
+        exact Nat.le_succ_of_le h
+      · cases' x with x
+        · simp [Subst.single, h₃, Term.level] at h''
+          exact Nat.not_succ_le_self _ h''
+        · simp [Subst.single, Term.level] at h''
+  · simp [Formula.level]
+    right
+    apply Nat.le_of_not_lt
+    intro h
+    apply Nat.le_of_lt_succ at h
+    apply Formula.level_of_subst_le at h
+    rcases h with ⟨_, h⟩
+    replace h := h _ h₄
+    simp [Subst.single, h₃, Term.level] at h
+
+lemma level_less_than_henkin_formula :
+  q ∈ 𝓛.HenkinFormulas → q.level ≤ p.level → q ≠ p → c ∉ q.consts := by
+  intros h₁' h₂' h₃' h₄'
+  rcases h₁' with ⟨q', c', m, q'', h₁'', h₂'', h₃'', h₄''⟩
+  simp [h₁'', Formula.consts, Formula.consts_of_subst] at h₄'
+  rcases h₄' with h₄' | ⟨x, h₄', h₅'⟩
+  · replace h₄' : n < q'.level := by
+      subst h₃; apply Formula.const_less_than_level; exact h₄'
+    have h₅' : q'.level ≤ m := by
+      subst h₂''; apply Formula.level_of_inj_omega
+    have h₆' : q.level = m + 1 :=
+      level_of_henkin_formula h₁'' h₂'' h₃'' h₄''
+    have h₇' : p.level = n + 1 :=
+      level_of_henkin_formula h₁ h₂ h₃ h₄
+    rw [h₆', h₇'] at h₂'
+    apply Nat.le_of_succ_le_succ at h₂'
+    exact Nat.not_le_of_lt (Nat.le_trans h₄' h₅') h₂'
+  · cases' x with x
+    · simp [Subst.single, Term.consts] at h₅'
+      subst h₃ h₃''
+      injection h₅' with h₅'
+      injection h₅' with h₅' h₅''
+      subst h₁ h₁'' h₂ h₂'' h₅' h₅''
+      contradiction
+    · simp [Term.consts] at h₅'
+
+end
+
+lemma consistency_of_henkin_formulas_aux {Γ : 𝓛.Context} :
+  Γ.Consistent → W ⊆ 𝓛.HenkinFormulas → Set.Finite W → (⌈Γ⌉ᴳ ∪ W).Consistent := by
+  intros h₁ h₂ h₃
+  let r : Formula 𝓛* → Formula 𝓛* → Prop := λ p q => p.level ≥ q.level
+  have : DecidableRel r := Classical.decRel r
+  have : IsTrans _ r := ⟨λ _ _ _ h₁ h₂ => Nat.le_trans h₂ h₁⟩
+  have : IsTotal _ r := ⟨λ _ _ => Nat.le_total _ _⟩
+  apply Set.Finite.induction_on_sorted (C := λ W => (⌈Γ⌉ᴳ ∪ W).Consistent) h₃ r
+  · simp; apply consts_keeps_consistency; exact h₁
+  · intros p W' h₄ h₅ h₆ h₇ h₈
+    simp; apply Context.Consistent.append.mpr
+    revert h₈; apply mt; intro h₈
+    rcases h₂ h₄ with ⟨p', c, n, p'', h₁', h₂', h₃', h₄'⟩
+    rw [h₁'] at h₈
+    apply Proof.mp
+    · exact Proof.mp Proof.not_imp_left h₈
+    · apply const_generalization (c := c)
+      · intros q h h'
+        cases' h with h h
+        · rcases h with ⟨q', h₁'', h₂''⟩
+          rw [←h₂'', h₃'] at h'
+          apply Formula.const_less_than_level at h'
+          rw [Formula.level_of_inj_consts] at h'
+          contradiction
+        · revert h'
+          apply level_less_than_henkin_formula h₁' h₂' h₃' h₄'
+          · exact h₂ (h₅ h)
+          · exact h₇ _ h
+          · intro h'; rw [h'] at h; contradiction
+      · intro h
+        simp [Formula.consts, h₃'] at h
+        apply Formula.const_less_than_level at h
+        apply Nat.not_le_of_lt at h
+        apply h
+        simp [h₂']
+        apply Formula.level_of_inj_omega
+      · exact Proof.mp Proof.not_imp_right h₈
+
+theorem consistency_of_henkin_formulas {Γ : 𝓛.Context} :
+  Γ.Consistent → (⌈Γ⌉ᴳ ∪ 𝓛.HenkinFormulas).Consistent := by
+  intros h₁ h₂
+  rcases Proof.compactness h₂ with ⟨Δ, ⟨h₂, ⟨h₃, h₄⟩⟩⟩
+  rcases Set.decompose_subset_union h₂ with ⟨Γ', W, h₅, h₆, h₇⟩
+  subst h₅
+  revert h₄
+  apply Context.Consistent.weaken
+  · apply Set.union_subset_union_left _ h₆
+  apply consistency_of_henkin_formulas_aux
+  · exact h₁
+  · exact h₇
+  · apply Set.Finite.subset
+    · exact h₃
+    · simp
+
+theorem henkin_formulas_saturated {Γ : (𝓛*).Context} :
+  𝓛.HenkinFormulas ⊆ Γ → Γ.Saturated := by
+  intros h₁ p h₂
+  by_cases h₃ : 0 ∈ p.free
+  · rcases Formula.exists_inj_omega (p := p) (le_refl _) with ⟨p', h⟩
+    let c : (𝓛*).Const := Sum.inr ⟨p.level, p'⟩
+    exists c
+    apply Proof.mp
+    · apply Proof.hyp
+      apply h₁
+      exists p, c, p.level, p'
+    · exact h₂
+  · exists Sum.inr ⟨0, (⊥ : Formula _)⟩
+    rw [←Formula.is_shift_iff] at h₃
+    rcases h₃ with ⟨p', h₃⟩
+    rw [h₃, Formula.shift_subst_single]
+    apply Proof.mp Proof.exists_self
+    rw [←h₃]
+    exact h₂
