MathematicalLogic/Vector.lean
@@ -1,0 +1,169 @@
+import Mathlib.Data.Vector.Basic
+import Mathlib.Data.Fin.Tuple.Basic
+import Mathlib.Data.Nat.Pairing
+
+@[elab_as_elim] def Fin.cases1 {motive : Fin 1 → Sort _}
+  (zero : motive 0) (i : Fin 1) : motive i := i.cases zero (·.elim0)
+@[elab_as_elim] def Fin.cases2 {motive : Fin 2 → Sort _}
+  (zero : motive 0) (one : motive 1) (i : Fin 2) : motive i :=
+  i.cases zero (λ i => i.cases one (·.elim0))
+@[elab_as_elim] def Fin.cases3 {motive : Fin 3 → Sort _}
+  (zero : motive 0) (one : motive 1) (two : motive 2)
+  (i : Fin 3) : motive i :=
+  i.cases zero (λ i => i.cases one (λ j => j.cases two (·.elim0)))
+
+def Vec (α : Type u) (n : ℕ) := Fin n → α
+
+namespace Vec
+
+variable {α : Type u}
+
+def nil : Vec α 0 := Fin.elim0
+def cons (a : α) (v : Vec α n) : Vec α (n + 1) := Fin.cons a v
+infixr:67 " ∷ᵥ " => cons
+syntax (name := vec) "[" term,* "]ᵥ" : term
+macro_rules
+| `([$t:term, $ts:term,*]ᵥ) => `(cons $t [$ts,*]ᵥ)
+| `([$t:term]ᵥ) => `(cons $t []ᵥ)
+| `([]ᵥ) => `(nil)
+
+@[simp] theorem cons_succ : (a ∷ᵥ v) i.succ = v i := rfl
+@[simp] theorem cons_0 : (a ∷ᵥ v) 0 = a := rfl
+@[simp] theorem cons_1 {v : Vec α (n + 1)} : (a ∷ᵥ v) 1 = v 0 := rfl
+@[simp] theorem cons_2 {v : Vec α (n + 2)} : (a ∷ᵥ v) 2 = v 1 := rfl
+@[simp] theorem cons_3 {v : Vec α (n + 3)} : (a ∷ᵥ v) 3 = v 2 := rfl
+
+@[app_unexpander nil] def unexpandNil : Lean.PrettyPrinter.Unexpander
+| `($(_)) => `([]ᵥ)
+
+@[app_unexpander cons] def unexpandCons : Lean.PrettyPrinter.Unexpander
+  | `($(_) $x $tail) =>
+    match tail with
+    | `([]ᵥ)      => `([$x]ᵥ)
+    | `([$xs,*]ᵥ) => `([$x, $xs,*]ᵥ)
+    | `(⋯)       => `([$x, $tail]ᵥ)
+    | _          => throw ()
+  | _ => throw ()
+
+@[ext] theorem ext {v₁ v₂ : Vec α n} :
+  (∀ i, v₁ i = v₂ i) → v₁ = v₂ := funext
+
+theorem ext_iff {v₁ v₂ : Vec α n} :
+  (∀ i, v₁ i = v₂ i) ↔ v₁ = v₂ := ⟨ext, congr_fun⟩
+
+def head (v : Vec α (n + 1)) := v 0
+@[simp] theorem head_cons : (a ∷ᵥ v).head = a := rfl
+def tail (v : Vec α (n + 1)) : Vec α n := v ∘ Fin.succ
+@[simp] theorem tail_app {v : Vec α (n + 1)} : v.tail x = v x.succ := rfl
+@[simp] theorem tail_cons : (a ∷ᵥ v).tail = v := rfl
+
+theorem cons_eq_iff : a₁ ∷ᵥ v₁ = a₂ ∷ᵥ v₂ ↔ a₁ = a₂ ∧ v₁ = v₂ := by
+  constructor
+  · intro h
+    rw [←head_cons (a := a₁), ←tail_cons (v := v₁), h]; simp
+  · intro ⟨h₁, h₂⟩
+    simp [h₁, h₂]
+
+theorem eq_nil (v : Vec α 0) : v = []ᵥ := by
+  ext x; exact x.elim0
+theorem eq_cons (v : Vec α (n + 1)) : v = v.head ∷ᵥ v.tail := by
+  ext x; cases x using Fin.cases <;> simp [cons, head, tail]
+theorem eq_1 (v : Vec α 1) : v = [v 0]ᵥ := by
+  rw [eq_cons v, eq_nil v.tail]; rfl
+theorem eq_2 (v : Vec α 2) : v = [v 0, v 1]ᵥ := by
+  rw [eq_cons v, eq_1 v.tail]; rfl
+theorem eq_3 (v : Vec α 3) : v = [v 0, v 1, v 2]ᵥ := by
+  rw [eq_cons v, eq_2 v.tail]; rfl
+theorem eq_4 (v : Vec α 4) : v = [v 0, v 1, v 2, v 3]ᵥ := by
+  rw [eq_cons v, eq_3 v.tail]; rfl
+
+section
+
+variable {motive : {n : ℕ} → Vec α n → Sort v}
+  (nil : motive []ᵥ)
+  (cons : {n : ℕ} → (a : α) → (v : Vec α n) → motive v → motive (a ∷ᵥ v))
+
+@[elab_as_elim] def rec : {n : ℕ} → (v : Vec α n) → motive v
+| 0, v => eq_nil v ▸ nil
+| (_ + 1), v => eq_cons v ▸ cons v.head v.tail (rec v.tail)
+@[simp] theorem rec_nil : rec nil cons []ᵥ = nil := rfl
+@[simp] theorem rec_cons : rec nil cons (a ∷ᵥ v) = cons a v (rec nil cons v) := rfl
+
+end
+
+@[simp] theorem comp_nil : f ∘ []ᵥ = []ᵥ := by ext x; exact x.elim0
+@[simp] theorem comp_cons : f ∘ (a ∷ᵥ v) = f a ∷ᵥ f ∘ v := by
+  ext x; cases x using Fin.cases <;> rfl
+theorem comp_comp {v : Vec α n} : g ∘ (f ∘ v) = (g ∘ f) ∘ v := rfl
+
+def rcons (v : Vec α n) (x : α) : Vec α (n + 1) := Fin.snoc v x
+@[simp] theorem rcons_nil : rcons []ᵥ x = [x]ᵥ := by
+  simp [rcons, Fin.snoc_zero]
+  ext i; cases i using Fin.cases1; simp
+@[simp] theorem rcons_cons : rcons (x ∷ᵥ v) y = x ∷ᵥ rcons v y := by
+  simp [rcons, Vec.cons, Fin.cons_snoc_eq_snoc_cons]
+
+def ofVector (v : Vector α n) : Vec α n := v.get
+def toVector (v : Vec α n) : Vector α n := .ofFn v
+
+instance decEq [DecidableEq α] : DecidableEq (Vec α n) := by
+  intro v₁ v₂
+  induction n with
+  | zero => rw [eq_nil v₁, eq_nil v₂]; exact isTrue rfl
+  | succ n ih =>
+    rw [eq_cons v₁, eq_cons v₂, cons_eq_iff]
+    have := ih v₁.tail v₂.tail
+    exact And.decidable
+
+def max : {n : ℕ} → Vec ℕ n → ℕ
+| 0, _ => 0
+| _ + 1, v => Nat.max v.head v.tail.max
+
+theorem le_max {v : Vec ℕ n} : v i ≤ v.max := by
+  induction n with
+  | zero => exact i.elim0
+  | succ n ih =>
+    cases i using Fin.cases with
+    | zero => apply Nat.le_max_left
+    | succ => rw [←tail_app (v := v)]; apply Nat.le_trans ih; apply Nat.le_max_right
+
+theorem max_le {v : Vec ℕ n} : (∀ i, v i ≤ m) → v.max ≤ m := by
+  intro h
+  induction n with simp [max]
+  | succ n ih =>
+    constructor
+    · apply h
+    · apply ih; intro; apply h
+
+theorem max_le_iff {v : Vec ℕ n} : v.max ≤ m ↔ ∀ i, v i ≤ m := by
+  constructor
+  · intro h i; exact le_trans le_max h
+  · exact max_le
+
+@[simp] theorem max_zero : max (n := n) (λ _ => 0) = 0 := by
+  apply Nat.eq_zero_of_le_zero
+  apply max_le
+  simp
+
+theorem max_eq_nth (v : Vec ℕ (n + 1)) : ∃ i, v.max = v i := by
+  induction n with
+  | zero => simp [max]; exists 0
+  | succ n ih =>
+    rw [max]
+    by_cases h : v.head ≤ v.tail.max
+    · simp [Nat.max_eq_right h]
+      rcases ih v.tail with ⟨i, h'⟩
+      exists i.succ
+    · simp [Nat.max_eq_left (Nat.le_of_not_ge h)]; exists 0
+
+theorem le_max_iff {v : Vec ℕ (n + 1)} : m ≤ v.max ↔ ∃ i, m ≤ v i := by
+  constructor
+  · intro h; rcases v.max_eq_nth with ⟨i, h'⟩; exists i; rw [←h']; exact h
+  · intro ⟨i, h⟩; apply le_trans h; exact le_max
+
+def paired : {n : ℕ} → Vec ℕ n → ℕ
+| 0, _ => 0
+| _ + 1, v => v.head.pair v.tail.paired
+
+end Vec
+
